More work on ARMv8 support, adding local state

ARMv8.thy
@@ -1,5 +1,5 @@
-theory ARMv8
-  imports Syntax
+theory ARMv82
+  imports Syntax Semantics
 begin
 
 chapter \<open>ARMv8\<close>
@@ -7,8 +7,8 @@ chapter \<open>ARMv8\<close>
 section \<open>State Encoding\<close>
 
 type_synonym ('v,'r) state = "(('v \<Rightarrow> 'v) \<times> ('r \<Rightarrow> 'v))"
-type_synonym ('v,'r) pred = "('v,'r) state \<Rightarrow> bool"
-type_synonym ('v,'r) rpred = "('v,'r) state \<Rightarrow> ('v,'r) state \<Rightarrow> bool"
+type_synonym ('v,'r) pred  = "('v,'r) state \<Rightarrow> bool"
+type_synonym ('v,'r) rpred = "('v \<Rightarrow> 'v) \<Rightarrow> ('v \<Rightarrow> 'v) \<Rightarrow> bool"
 
 named_theorems pred_defs
 definition conj  (infixr "\<and>\<^sub>p" 35)
@@ -36,8 +36,8 @@ abbreviation PTrue
 
 subsection \<open>Write Operations\<close>
 
-definition pair_upd1 :: "(('v \<Rightarrow> 'v) \<times> ('c \<Rightarrow> 'v)) \<Rightarrow> 'c \<Rightarrow> 'v \<Rightarrow> (('v \<Rightarrow> 'v) \<times> ('c \<Rightarrow> 'v))"
-  where "pair_upd1 f a b = (\<lambda>x. if x = snd f a then b else (fst f) x, snd f)"
+definition pair_upd1 :: "(('v \<Rightarrow> 'v) \<times> ('c \<Rightarrow> 'v)) \<Rightarrow> 'v \<Rightarrow> 'v \<Rightarrow> (('v \<Rightarrow> 'v) \<times> ('c \<Rightarrow> 'v))"
+  where "pair_upd1 f a b = (\<lambda>x. if x = a then b else (fst f) x, snd f)"
 
 definition pair_upd2 :: "(('a \<Rightarrow> 'b) \<times> ('c \<Rightarrow> 'd)) \<Rightarrow> 'c \<Rightarrow> 'd \<Rightarrow> (('a \<Rightarrow> 'b) \<times> ('c \<Rightarrow> 'd))"
   where "pair_upd2 f a b = (fst f, \<lambda>x. if x = a then b else (snd f) x)"
@@ -59,194 +59,101 @@ translations
 subsection \<open>Read Operations\<close>
 
 abbreviation rg
-  where "rg r m \<equiv> (snd m) r"
+  where "rg m r \<equiv> (snd m) r"
 
 abbreviation ld
-  where "ld x m \<equiv> (fst m) (snd m x)"
+  where "ld m x \<equiv> (fst m) x"
 
-section \<open>Instruction Language Definition\<close>
+section \<open>Sub-Instruction Language Definition\<close>
 
-text \<open>Capture a simple set of instructions, covering memory operations and fences\<close>
-(* TODO: Need support for CAS and other RMW *)
+text \<open>Capture a simple set of sub-instructions, covering memory operations and fences\<close>
 datatype ('v,'r) inst =
-    Load1 'r 'v
-  | Load2 'r 'r 'v
-  | Store 'r 'r
-  | Op 'r "'v \<Rightarrow> 'v \<Rightarrow> 'v" 'r 'r
-  | Cond "'v \<Rightarrow> bool" 'r
-  | Fence
-  | CFence
-  | StFence
+    load 'v 'v
+  | store 'v 'r
+  | cas 'v 'v 'v
+  | op 'r "'v list \<Rightarrow> 'v" "'r list"
+  | test "'v list \<Rightarrow> bool" "'r list"
+  | fence
+  | cfence
+  | stfence
 
-text \<open>Shorthand for a negative condition\<close>
-abbreviation NCond
-  where "NCond f r \<equiv> Cond (\<lambda>v. \<not> f v) r"
-
-text \<open>Instruction Behaviour\<close>
+text \<open>Sub-Instruction Behaviour\<close>
 fun beh\<^sub>i :: "('v,'r) inst \<Rightarrow> ('v,'r) state rel"
   where
-    "beh\<^sub>i (Store x r) = {(m,m'). m' = m (x :=\<^sub>1 rg r m)}" |
-    "beh\<^sub>i (Load1 y v) = {(m,m'). m' = m  \<and> v = ld y m}" |
-    "beh\<^sub>i (Load2 r y v) = {(m,m'). m' = m (r :=\<^sub>2 v)}" |
-    "beh\<^sub>i (Op r\<^sub>t f r\<^sub>1 r\<^sub>2) = {(m,m'). m' = m (r\<^sub>t :=\<^sub>2 f (rg r\<^sub>1 m) (rg r\<^sub>2 m))}" |
-    "beh\<^sub>i (Cond f r) = {(m,m'). m = m' \<and> f (rg r m)}" |
+    "beh\<^sub>i (store addr r) = {(m,m'). m' = m (addr :=\<^sub>1 rg m r)}" |
+    "beh\<^sub>i (load addr val) = {(m,m'). m' = m \<and> ld m addr = val}" |
+    "beh\<^sub>i (cas addr tst val) = {(m,m'). (m' = m \<and> ld m addr \<noteq> tst) \<or> (m' = m (addr :=\<^sub>1 val) \<and> ld m addr = tst)}" |
+    "beh\<^sub>i (op r f rs) = {(m,m'). m' = m (r :=\<^sub>2 f (map (rg m) rs))}" |
+    "beh\<^sub>i (test f rs) = {(m,m'). m = m' \<and> f (map (rg m) rs)}" |
     "beh\<^sub>i _ = Id"
 
-subsection \<open>Reordering\<close>
-
-(*
-text \<open>Define forwarding as the elimination of loads given a store to the same address\<close>
-fun fwd :: "('v,'r) inst \<Rightarrow> ('v,'r) inst \<Rightarrow> ('v,'r) inst" 
-  ("_\<langle>_\<rangle>" [1000,0] 1000)
-  where 
-    "fwd (Load r\<^sub>2 y) (Store x r\<^sub>1) = (if (x = y) then Op r\<^sub>2 (\<lambda>x y. x) r\<^sub>1 r\<^sub>1 else Load r\<^sub>2 y)" |
-    "fwd \<alpha> _ = \<alpha>" *)
-
-fun reads
+text \<open>Sub-Instruction Reordering\<close>
+fun re\<^sub>i :: "('v,'r) inst \<Rightarrow> ('v,'r) inst \<Rightarrow> bool" 
   where
-    "reads (Store x r) = {x,r}" |
-    "reads (Load1 y v) = {y}" |
-    "reads (Load2 r y v) = {r,y}" |
-    "reads (Op _ _ r\<^sub>1 r\<^sub>2) = {r\<^sub>1,r\<^sub>2}" |
-    "reads (Cond _ r) = {r}" |
-    "reads _ = {}"
+    "re\<^sub>i _ fence = False" |
+    "re\<^sub>i fence _ = False" |
+    "re\<^sub>i (store _ _) stfence = False" |
+    "re\<^sub>i stfence (store _ _) = False" | 
+    "re\<^sub>i (test _ _) cfence = False" |
+    "re\<^sub>i cfence (load _ _) = False" |
+    "re\<^sub>i (load y _) (load x _) = (y \<noteq> x)" |
+    "re\<^sub>i (load y _) (store x _) = (y \<noteq> x)" |
+    "re\<^sub>i (store x _) (load y _) = (y \<noteq> x)" |
+    "re\<^sub>i (store x _) (store y _) = (y \<noteq> x)" |
+    "re\<^sub>i (store _ r) (op r' _ _) = (r \<noteq> r')" |
+    "re\<^sub>i (op r _ rs) (op r' _ rs') = (r \<notin> set rs' \<and> r' \<notin> set rs \<and> r \<noteq> r')" |
+    "re\<^sub>i (op r _ _) (test _ rs') = (r \<notin> set rs')" |
+    "re\<^sub>i (op r _ _) (store _ r') = (r \<noteq> r')" |
+    "re\<^sub>i (test _ _) (store _ _) = False" |
+    "re\<^sub>i (test _ rs) (op r _ _) = (r \<notin> set rs)" |
+    "re\<^sub>i _ _ = True"
 
-fun writes
+text \<open>Sub-Instruction Forwarding\<close>
+fun fwd\<^sub>i :: "('v,'r) inst \<Rightarrow> ('v,'r) inst \<Rightarrow> ('v,'r) inst" 
   where
-    "writes (Op r _ _ _) = {r}" |
-    "writes (Load2 r _ _) = {r}" |
-    "writes _ = {}"
+    "fwd\<^sub>i (load v\<^sub>a v) (store v\<^sub>a' r) = (if v\<^sub>a = v\<^sub>a' then test (\<lambda>x. x ! 0 = v) [r] else load v\<^sub>a v)" |
+    "fwd\<^sub>i \<alpha> _ = \<alpha>"
 
-fun addrs
-  where
-    "addrs (Store x _) = {x}" |
-    "addrs (Load1 y _) = {y}" |
-    "addrs _ = {}"
+text \<open>Common Sub-Instructions\<close>
+abbreviation eq
+  where "eq r v \<equiv> test (\<lambda>x. x ! 0 = v) [r]"
 
-fun re :: "('v,'r) inst \<Rightarrow> ('v,'r) inst \<Rightarrow> bool" 
-  where
-    "re _ Fence = False" |
-    "re Fence _ = False" |
-    "re (Store _ _) StFence = False" |
-    "re StFence (Store _ _) = False" | 
-    "re (Cond _ _) CFence = False" |
-    "re CFence (Load1 _ _) = False" |
+abbreviation assign
+  where "assign r v \<equiv> op r (\<lambda>x. v) []"
 
-    "re (Cond _ _) (Store _ _) = False" |
-    "re (Cond _ r\<^sub>c) (Op r\<^sub>t _ r\<^sub>1 r\<^sub>2) = (r\<^sub>c \<noteq> r\<^sub>t)" |
-    "re (Cond _ r\<^sub>c) (Load2 r\<^sub>t _ _) = (r\<^sub>c \<noteq> r\<^sub>t)" |
+abbreviation ntest
+  where "ntest f rs \<equiv> test (\<lambda>x. \<not> f x) rs"
 
-    "re (Store x r\<^sub>s) (Load2 r\<^sub>t _ _) = (r\<^sub>s \<noteq> r\<^sub>t \<and> x \<noteq> r\<^sub>t)" |
-    "re (Store x r\<^sub>s) (Op r\<^sub>t _ r\<^sub>1 r\<^sub>2) = (r\<^sub>s \<noteq> r\<^sub>t \<and> x \<noteq> r\<^sub>t)" |
-
-    "re (Load1 y _) (Load2 r\<^sub>t x _) = (y \<noteq> x \<and> r\<^sub>t \<noteq> y)" |
-    "re (Load1 y _) (Op r\<^sub>t _ r\<^sub>1 r\<^sub>2) = (y \<noteq> r\<^sub>t)" |
-
-    "re (Load2 r\<^sub>t x _) (Load1 y _) = (y \<noteq> x \<and> r\<^sub>t \<noteq> y)" |
-    "re (Load2 r\<^sub>t y _) (Load2 r\<^sub>t' x _) = (r\<^sub>t \<noteq> r\<^sub>t' \<and> r\<^sub>t \<noteq> x \<and> r\<^sub>t' \<noteq> y)" |
-    "re (Load2 r\<^sub>t _ _) (Store x r\<^sub>s) = (r\<^sub>s \<noteq> r\<^sub>t \<and> x \<noteq> r\<^sub>t)" |
-    "re (Load2 r\<^sub>t y _) (Op r\<^sub>t' _ r\<^sub>1 r\<^sub>2) = (r\<^sub>t \<noteq> r\<^sub>t' \<and> r\<^sub>t' \<noteq> y \<and> r\<^sub>t \<noteq> r\<^sub>1 \<and> r\<^sub>t \<noteq> r\<^sub>2)" |
-    "re (Load2 r\<^sub>t _ _) (Cond _ r\<^sub>s) = (r\<^sub>t \<noteq> r\<^sub>s)" |
-
-    "re (Op r\<^sub>t _ r\<^sub>1 r\<^sub>2) (Load1 y _) = (y \<noteq> r\<^sub>t)" |
-    "re (Op r\<^sub>t _ r\<^sub>1 r\<^sub>2) (Load2 r\<^sub>t' y _) = (r\<^sub>t' \<noteq> r\<^sub>t \<and> r\<^sub>t' \<noteq> r\<^sub>1 \<and> r\<^sub>t' \<noteq> r\<^sub>2 \<and> r\<^sub>t \<noteq> y)" |
-
-    "re (Op r\<^sub>t _ r\<^sub>1 r\<^sub>2) (Store x r\<^sub>s) = (r\<^sub>t \<noteq> r\<^sub>s \<and> r\<^sub>t \<noteq> x)" |
-    "re (Op r\<^sub>t _ r\<^sub>1 r\<^sub>2) (Op r\<^sub>t' _ r\<^sub>1' r\<^sub>2') = (r\<^sub>t' \<noteq> r\<^sub>t \<and> r\<^sub>t' \<noteq> r\<^sub>1 \<and> r\<^sub>t' \<noteq> r\<^sub>2 \<and> r\<^sub>t \<noteq> r\<^sub>1' \<and> r\<^sub>t \<noteq> r\<^sub>2')" |
-    "re (Op r\<^sub>t _ r\<^sub>1 r\<^sub>2) (Cond _ r\<^sub>s) = (r\<^sub>t \<noteq> r\<^sub>s)" |
-
-    "re _ _ = True"
-
-lemma
-  "re \<alpha> \<beta> \<Longrightarrow> writes \<alpha> \<inter> writes \<beta> = {}"
-  by (cases \<alpha>; cases \<beta>; auto)
-
-lemma
-  "re \<alpha> \<beta> \<Longrightarrow> writes \<alpha> \<inter> reads \<beta> = {}"
-  by (cases \<alpha>; cases \<beta>; auto)
-
-lemma
-  "re \<alpha> \<beta> \<Longrightarrow> reads \<alpha> \<inter> writes \<beta> = {}"
-  by (cases \<alpha>; cases \<beta>; auto)
-
-
-
-text \<open>Define reordering based on Colvin & Smith\<close>
-fun re_m :: "('v,'r) inst \<Rightarrow> ('v,'r) inst \<Rightarrow> ('v,'r) pred" 
-  where
-    "re_m (Store y _) (Load1 x _) = (\<lambda>m. rg x m \<noteq> rg y m)" |
-    "re_m (Store y _) (Store x _) = (\<lambda>m. rg x m \<noteq> rg y m)" |
-    "re_m (Load1 y _) (Store x _) = (\<lambda>m. rg x m \<noteq> rg y m)" |
-    "re_m _ _ = PTrue"
-
-section \<open>Instruction Specification Language Definition\<close>
+section \<open>Sub-Instruction Specification Language\<close>
 
 text \<open>Wrap instructions in more abstract specification to facilitate verification\<close>
-type_synonym ('v,'r) ispec = "(('v,'r) pred \<times> ('v,'r) pred \<times> ('v,'r) inst)"
+type_synonym ('v,'r) ispec = "(('v,'r) pred \<times> ('v,'r) inst)"
 
 text \<open>Duplicate forwarding and reordering behaviour of underlying instruction\<close>
 fun fwd\<^sub>s :: "('v,'r) ispec \<Rightarrow> ('v,'r) ispec \<Rightarrow> ('v,'r) ispec" 
-  where 
-    "fwd\<^sub>s (vc,ts,\<alpha>) (_,_,\<beta>) = (if re \<beta> \<alpha> then (vc,ts \<and>\<^sub>p re_m \<beta> \<alpha>,\<alpha>) else (vc,PFalse,\<alpha>))" 
+  where "fwd\<^sub>s (vc,\<alpha>) (_,\<beta>) =  (vc,fwd\<^sub>i \<alpha> \<beta>)" 
 
 fun beh\<^sub>s :: "('v,'r) ispec \<Rightarrow> ('v,'r) state rel" 
-  where "beh\<^sub>s (_,ts,\<alpha>) = {(m,m'). (m,m') \<in> beh\<^sub>i \<alpha>}" 
+  where "beh\<^sub>s (_,\<alpha>) = beh\<^sub>i \<alpha>" 
 
 fun vc\<^sub>s :: "('v,'r) ispec \<Rightarrow> ('v,'r) state set" 
-  where "vc\<^sub>s (p,ts,\<alpha>) = {m. ts m \<longrightarrow> p m}" 
+  where "vc\<^sub>s (p,\<alpha>) = Collect p" 
 
-(* does ts\<^sub>\<alpha> depend on writes in \<beta>? *)
+abbreviation no_vc ("\<lfloor>_\<rfloor>" 100)
+  where "no_vc \<alpha> \<equiv> (\<lambda>x. True, \<alpha>)"
 
-definition comp (infixr "\<otimes>" 60)
-  where "comp a b \<equiv> {((g,l),(g',l')). (\<exists>g'' l'' . ((g,l),(g'',l'')) \<in> a \<and> ((g'',l''),(g',l')) \<in> b)}"
-
-lemma
-  "re (snd (snd \<alpha>))  (snd (snd \<beta>)) \<Longrightarrow> beh\<^sub>s \<alpha> \<otimes> beh\<^sub>s \<beta> \<supseteq> {((g,l),(g',l')). (re_m (snd (snd \<alpha>))  (snd (snd \<beta>))) (g,l) \<and> g = g' \<and> l = l' } \<otimes> beh\<^sub>s (fwd\<^sub>s \<beta> \<alpha>) \<otimes> beh\<^sub>s \<alpha>"
-  apply (cases \<alpha>; cases \<beta>)
-  apply (case_tac c; case_tac ca)
-  by (auto simp: pred_defs pair_upd1_def pair_upd2_def comp_def split: if_splits)
-
-
-(*
-  apply (rename_tac vc\<^sub>\<alpha> ts\<^sub>\<alpha> a vc\<^sub>\<beta> ts\<^sub>\<beta> b x v r\<^sub>2 y v')
-  apply (auto simp: pred_defs comp_def pair_upd2_def)[1]
-  defer 1
-  apply (auto simp: pred_defs comp_def pair_upd1_def pair_upd2_def)[1]
-  defer 1
-  apply (auto simp: pred_defs comp_def pair_upd1_def pair_upd2_def)[1]
-  defer 1
-  apply (auto simp: pred_defs comp_def pair_upd1_def pair_upd2_def)[1]
-  apply (auto simp: pred_defs comp_def pair_upd1_def pair_upd2_def)[1]
-  apply (auto simp: pred_defs comp_def pair_upd1_def pair_upd2_def)[1]
-  apply (auto simp: pred_defs comp_def pair_upd1_def pair_upd2_def)[1]
-  apply (auto simp: pred_defs comp_def pair_upd1_def pair_upd2_def)[1]
-*)
-
-
-
-text \<open>Common case of a true verification condition\<close>
-abbreviation VC\<^sub>T
-  where "VC\<^sub>T \<alpha> \<equiv> (PTrue,PTrue,\<alpha>)"
+abbreviation yes_vc ("\<lfloor>_,_\<rfloor>" 100)
+  where "yes_vc v \<alpha> \<equiv> (v, \<alpha>)"
 
 section \<open>While Language Definition\<close>
 
 datatype ('v,'r) lang =
-    Skip
-  | Inst "('v,'r) ispec"
+  Skip
+  | Load "('v,'r) pred" 'r 'r
+  | Store "('v,'r) pred" 'r 'r
+  | Op 'r "'v list \<Rightarrow> 'v" "'r list"
   | Seq "('v,'r) lang" "('v,'r) lang"
-  | If "'v \<Rightarrow> bool" 'r "('v,'r) lang" "('v,'r) lang"
-  | While "'v \<Rightarrow> bool" 'r "('v,'r) pred" "('v,'r) lang"
-
-text \<open>Convert the While language into the com language expected by the underlying logic\<close> 
-(* TODO: This should be later, closer to the soundness proof *)
-fun lift\<^sub>c :: "('v,'r) lang \<Rightarrow> (('v,'r) ispec,('v,'r) state) com"
-  where
-    "lift\<^sub>c Skip = com.Nil" |
-    "lift\<^sub>c (Inst \<alpha>) = Basic \<alpha>"|
-    "lift\<^sub>c (Seq c\<^sub>1 c\<^sub>2) = (com.Seq (lift\<^sub>c c\<^sub>1) (lift\<^sub>c c\<^sub>2))" |
-    "lift\<^sub>c (If f r c\<^sub>1 c\<^sub>2) = (Choice (com.Seq (Basic (VC\<^sub>T (Cond f r))) (lift\<^sub>c c\<^sub>1)) 
-                                    (com.Seq (Basic (VC\<^sub>T (NCond f r))) (lift\<^sub>c c\<^sub>2)))" |
-    "lift\<^sub>c (While f r I c) = (com.Seq ((com.Seq (Basic (VC\<^sub>T (Cond f r))) (lift\<^sub>c c))*) 
-                                      (Basic (VC\<^sub>T (NCond f r))))"
+  | If "'v list \<Rightarrow> bool" "'r list" "('v,'r) lang" "('v,'r) lang"
+  | While "'v list \<Rightarrow> bool" "'r list" "('v,'r) pred" "('v,'r) lang"
 
 end
