Atomics.thy
@@ -10,12 +10,36 @@ Describe concepts the logic must know about atomic instructions.
 
 section \<open>Helper Definitions\<close>
 
-type_synonym 'b pred = "'b set"
-type_synonym 'b rpred = "'b rel"
+datatype 'c tree = Leaf 'c | Branch "'c tree" "'c tree"
+
+type_synonym ('b,'c) gpred = "('b \<times> 'c tree) set"
+type_synonym ('b,'c) pred = "('b \<times> 'c) set"
+type_synonym ('b,'c) rpred = "'b rel"
+
+definition leaf :: "('b \<times> 'c) set \<Rightarrow> ('b \<times> 'c tree) set"
+  where "leaf e \<equiv> {(g,Leaf l) | g l. (g,l) \<in> e}"
+
+definition left :: "('b \<times> 'c tree) set \<Rightarrow> ('b \<times> 'c tree) set"
+  where "left e \<equiv> {(g,Branch l r) | g l r. (g,l) \<in> e}"
+
+definition right :: "('b \<times> 'c tree) set \<Rightarrow> ('b \<times> 'c tree) set"
+  where "right e \<equiv> {(g,Branch l r) | g l r. (g,r) \<in> e}"
+
+definition leaf\<^sub>r :: "('b \<times> 'c) rel \<Rightarrow> ('b \<times> 'c tree) rel"
+  where "leaf\<^sub>r e \<equiv> {((g,Leaf l),(g', Leaf l')) | g g' l l'. ((g,l),(g',l')) \<in> e}"
+
+definition left\<^sub>r :: "('b \<times> 'c tree) rel \<Rightarrow> ('b \<times> 'c tree) rel"
+  where "left\<^sub>r e \<equiv> {((g,Branch l r),(g',Branch l' r)) | g g' l l' r. ((g,l),(g',l')) \<in> e}"
+
+definition right\<^sub>r :: "('b \<times> 'c tree) rel \<Rightarrow> ('b \<times> 'c tree) rel"
+  where "right\<^sub>r e \<equiv> {((g,Branch l r),(g', Branch l r')) | g g' l r r'. ((g,r),(g',r')) \<in> e}"
+
+definition any :: "('b) set \<Rightarrow> ('b \<times> 'c tree) set"
+  where "any e \<equiv> {(g,t) | t g. (g) \<in> e}"
 
 text \<open>Stability of a predicate across an environment step\<close>
-definition stable :: "'a rel \<Rightarrow> 'a set \<Rightarrow> bool"
-  where "stable R P \<equiv> \<forall>m m'. m \<in> P \<longrightarrow> (m,m') \<in> R \<longrightarrow> m' \<in> P"
+definition stable :: "('b,'c) rpred \<Rightarrow> ('b,'c) pred \<Rightarrow> bool"
+  where "stable R P \<equiv> \<forall>g l g'. (g,l) \<in> P \<longrightarrow> (g,g') \<in> R \<longrightarrow> (g',l) \<in> P"
 
 text \<open>Weakest precondition for a precondition and postrelation\<close>
 definition wp 
@@ -34,31 +58,35 @@ lemma stable_conjI [intro]:
   using assms by (auto simp: stable_def)
 
 lemma stable_transitive:
-  assumes "(m,m') \<in> R\<^sup>*" "m \<in> P" "stable R P"
-  shows "m' \<in> P"
+  assumes "(g,g') \<in> R\<^sup>*" "(g,l) \<in> P" "stable R P"
+  shows "(g',l) \<in> P"
   using assms by (induct rule: rtrancl.induct) (auto simp: stable_def)
 
 lemma stable_wp\<^sub>tI:
-  "stable R P \<Longrightarrow> P \<subseteq> wp UNIV (R\<^sup>* ) P"
+  "stable R P \<Longrightarrow> P \<subseteq> wp UNIV (fullR (R\<^sup>*)) P"
   unfolding wp_def using stable_transitive by fast
+
+lemma [intro]:
+  "stable R {}"
+  by (auto simp: stable_def)
 
 section \<open>Atomic Properties\<close>
 
 locale atomic =
-  fixes vc :: "'a \<Rightarrow> 'b set"
-  and beh :: "'a \<Rightarrow> 'b rel"
+  fixes vc :: "'a \<Rightarrow> ('b \<times> 'c) set"
+  and beh :: "'a \<Rightarrow> ('b \<times> 'c) rel"
 
 context atomic
 begin
 
 text \<open>Weakest precondition of a basic instruction, based on the locale's 
       verification conditions and behaviours.\<close>
-abbreviation wp\<^sub>\<alpha> :: "'a \<Rightarrow> 'b set \<Rightarrow> 'b set"
+abbreviation wp\<^sub>\<alpha> :: "'a \<Rightarrow> ('b,'c) pred \<Rightarrow> ('b,'c) pred"
   where "wp\<^sub>\<alpha> \<alpha> Q \<equiv> wp (vc \<alpha>) (beh \<alpha>) Q"
 
 text \<open>Weakest precondition of a program, only covering basic instructions, environment steps and 
       sequential composition as these are sufficient for the logic's checks.\<close>
-fun wp\<^sub>c :: "('a,'b) com \<Rightarrow> 'b set \<Rightarrow> 'b set"
+fun wp\<^sub>c :: "('a,'b,'c) com \<Rightarrow> ('b,'c) pred \<Rightarrow> ('b,'c) pred"
   where 
     "wp\<^sub>c (Basic \<alpha>) Q = wp\<^sub>\<alpha> \<alpha> Q" |
     "wp\<^sub>c (Rel r) Q = wp UNIV r Q" |
@@ -66,16 +94,16 @@ fun wp\<^sub>c :: "('a,'b) com \<Rightarrow> 'b set \<Rightarrow> 'b set"
     "wp\<^sub>c _ Q = undefined"
 
 text \<open>Refinement relation between two programs, in terms of their weakest precondition calculation.\<close>
-definition refine :: "('a,'b) com \<Rightarrow> ('a,'b) com \<Rightarrow> bool" (infix "\<sqsubseteq>" 60)
+definition refine :: "('a,'b,'c) com \<Rightarrow> ('a,'b,'c) com \<Rightarrow> bool" (infix "\<sqsubseteq>" 60)
   where "c \<sqsubseteq> c' \<equiv> \<forall>Q. wp\<^sub>c c Q \<subseteq> wp\<^sub>c c' Q"
 
 text \<open>Merge the verification condition and behaviour to define evaluation\<close>
-definition eval :: "'a \<Rightarrow> 'b rpred"
+definition eval :: "'a \<Rightarrow> ('b \<times> 'c) rel"
   where "eval \<alpha> \<equiv> {(m,m'). m \<in> vc \<alpha> \<longrightarrow> (m,m') \<in> beh \<alpha>}"
 
 text \<open>Specification check, ensuring an instruction conforms to a relation\<close>
-abbreviation guar :: "'a \<Rightarrow> 'b rpred \<Rightarrow> bool"
-  where "guar \<alpha> G \<equiv> {(m,m'). m \<in> vc \<alpha>} \<inter> beh \<alpha> \<subseteq> G\<^sup>="
+abbreviation guar :: "'a \<Rightarrow> ('b,'c) rpred \<Rightarrow> bool"
+  where "guar \<alpha> G \<equiv> {(g,g'). \<exists>l l'. (g,l) \<in> vc \<alpha> \<and> ((g,l),(g',l')) \<in> beh \<alpha>} \<subseteq> G\<^sup>="
 
 end
 
@@ -87,7 +115,7 @@ context atomic_rule
 begin
 
 text \<open>Rule for an atomic operation\<close>
-definition atomic_rule :: "'b rpred \<Rightarrow> 'b rpred \<Rightarrow> 'b pred \<Rightarrow> 'a \<Rightarrow> 'b pred \<Rightarrow> bool" 
+definition atomic_rule :: "('b,'c) rpred \<Rightarrow> ('b,'c) rpred \<Rightarrow> ('b,'c) pred \<Rightarrow> 'a \<Rightarrow> ('b,'c) pred \<Rightarrow> bool" 
   ("_,_ \<turnstile>\<^sub>A _ {_} _" [40,0,0,0,40] 40)
   where "R,G \<turnstile>\<^sub>A P {\<alpha>} Q \<equiv> P \<subseteq> wp\<^sub>\<alpha> \<alpha> Q \<and> guar \<alpha> G \<and> stable R P \<and> stable R Q"
 
@@ -97,23 +125,21 @@ text \<open>Re-establish an atomic judgement over a stronger stable precondition
 lemma atomic_pre:
   assumes "R,G \<turnstile>\<^sub>A P {\<alpha>} Q" "P' \<subseteq> P" "stable R P'"
   shows "R,G \<turnstile>\<^sub>A P' {\<alpha>} Q"
-  using assms unfolding atomic_rule_def
-  by fast
+  using assms unfolding atomic_rule_def by fast
 
 text \<open>Strengthen the rely and weaken the guarantee for an atomic judgement\<close>
 lemma atomic_conseqI [intro]:
   assumes "R,G \<turnstile>\<^sub>A P {\<alpha>} Q" "R' \<subseteq> R" "G \<subseteq> G'"
   shows "R',G' \<turnstile>\<^sub>A P {\<alpha>} Q"
-  using assms unfolding atomic_rule_def
-  by blast
+  using assms unfolding atomic_rule_def by blast
 
 text \<open>Atomic judgements over the same instruction can be combined\<close>
 lemma actomic_conjI [intro]:
   assumes "R,G \<turnstile>\<^sub>A P\<^sub>1 {\<alpha>} Q\<^sub>1" "R,G  \<turnstile>\<^sub>A P\<^sub>2 {\<alpha>} Q\<^sub>2"
   shows "R,G \<turnstile>\<^sub>A P\<^sub>1 \<inter> P\<^sub>2 {\<alpha>} Q\<^sub>1 \<inter> Q\<^sub>2"
-  using assms unfolding atomic_rule_def wp_def stable_def
-  by fast
+  using assms unfolding atomic_rule_def wp_def stable_def by fast
 
+(*
 text \<open>Add an invariant across an atomic judgement\<close>
 lemma atomic_frameI [intro]:
   assumes "R,G \<turnstile>\<^sub>A P {\<alpha>} Q"
@@ -121,13 +147,14 @@ lemma atomic_frameI [intro]:
   shows "R \<inter> R\<^sub>2,G \<turnstile>\<^sub>A P \<inter> M {\<alpha>} Q \<inter> M"
   unfolding atomic_rule_def
 proof (safe, goal_cases)
-  case (1 x)
-  hence "{(m,m'). m \<in> P \<inter> vc \<alpha>} \<inter> beh \<alpha> \<subseteq> R\<^sub>2\<^sup>=" "x \<in> vc \<alpha>"
+  case (1 g l)
+  hence "{(g,g'). \<exists>l l'. (g,l) \<in> P \<inter> vc \<alpha> \<and> ((g,l),(g',l')) \<in> beh \<alpha>} \<subseteq> R\<^sub>2\<^sup>=" "(g,l) \<in> vc \<alpha>"
     using assms(1,3) by (auto simp: wp_def atomic_rule_def)
-  hence "x \<in> wp\<^sub>\<alpha> \<alpha> M" using assms(2) 1 by (auto simp: wp_def stable_def)
-  moreover have "x \<in> wp\<^sub>\<alpha> \<alpha> Q" using 1 assms(1) by (auto simp: atomic_rule_def wp_def)
+  hence "(g,l) \<in> wp\<^sub>\<alpha> \<alpha> M" using assms(2) 1 by (auto simp: wp_def stable_def)
+  moreover have "(g,l) \<in> wp\<^sub>\<alpha> \<alpha> Q" using 1 assms(1) by (auto simp: atomic_rule_def wp_def)
   ultimately show ?case by (auto simp: wp_def)
 qed (insert assms, auto simp: atomic_rule_def wp_def)
+*)
 
 end
 
