Global_Rules.thy
@@ -6,8 +6,6 @@ chapter \<open>Global Rules\<close>
 
 text \<open>Define the rely/guarantee rules for a concurrent program.\<close>
 
-print_locale interference
-
 locale global_rules = interference + local_rules
 
 context global_rules
@@ -16,15 +14,15 @@ begin
 section \<open>Global Rules\<close>
 
 text \<open>Establish the rules of the logic, similar to standard Hoare-logic\<close>
-inductive rules :: "'b rpred \<Rightarrow> 'b rpred \<Rightarrow> 'b pred \<Rightarrow> ('a,'b) com \<Rightarrow> 'b pred \<Rightarrow> bool" 
+inductive rules :: "('b,'c) rpred \<Rightarrow> ('b,'c) rpred \<Rightarrow> ('b \<times> 'c tree) set \<Rightarrow> ('a,'b,'c) com \<Rightarrow> ('b \<times> 'c tree) set \<Rightarrow> bool" 
   ("_,_ \<turnstile> _ {_} _" [20,0,0,0,20] 20)
 where
-  thread[intro]: "R,G \<turnstile>\<^sub>l P { c } Q \<Longrightarrow> inter R G c \<Longrightarrow> R,G \<turnstile> P { c } Q" |
+  thread[intro]: "R,G \<turnstile>\<^sub>l P { c } Q \<Longrightarrow> inter R G c \<Longrightarrow> R,G \<turnstile> leaf P { c } leaf Q" |
   par[intro]:    "R\<^sub>1,G\<^sub>1 \<turnstile> P\<^sub>1 { c\<^sub>1 } Q\<^sub>1 \<Longrightarrow> R\<^sub>2,G\<^sub>2 \<turnstile> P\<^sub>2 { c\<^sub>2 } Q\<^sub>2 \<Longrightarrow> G\<^sub>2 \<subseteq> R\<^sub>1 \<Longrightarrow> G\<^sub>1 \<subseteq> R\<^sub>2 \<Longrightarrow> 
-                  R\<^sub>1 \<inter> R\<^sub>2,G\<^sub>1 \<union> G\<^sub>2 \<turnstile> P\<^sub>1 \<inter> P\<^sub>2 { c\<^sub>1 || c\<^sub>2 } (Q\<^sub>1 \<inter> Q\<^sub>2)" |
+                  R\<^sub>1 \<inter> R\<^sub>2,G\<^sub>1 \<union> G\<^sub>2 \<turnstile> left P\<^sub>1 \<inter> right P\<^sub>2 { c\<^sub>1 || c\<^sub>2 } (left Q\<^sub>1 \<inter> right Q\<^sub>2)" |
   conseq[intro]: "R,G \<turnstile> P { c } Q \<Longrightarrow> P' \<subseteq> P \<Longrightarrow> R' \<subseteq> R \<Longrightarrow> G \<subseteq> G' \<Longrightarrow> Q \<subseteq> Q' \<Longrightarrow> 
-                  R',G' \<turnstile> P' { c } Q'" |
-  frame[intro]:  "R,G \<turnstile> P {c} Q \<Longrightarrow> stable R' M \<Longrightarrow> G \<subseteq> R' \<Longrightarrow> R \<inter> R',G \<turnstile> P \<inter> M {c} Q \<inter> M"
+                  R',G' \<turnstile> P' { c } Q'"  |
+  frame[intro]:  "R,G \<turnstile> P {c} Q \<Longrightarrow> stable R' (any M :: ('b \<times> 'c tree) set) \<Longrightarrow> G \<subseteq> R' \<Longrightarrow> R \<inter> R',G \<turnstile> (P \<inter> any M) {c} (Q \<inter> any M)"
 
 subsection \<open>Properties\<close>
 
@@ -32,11 +30,11 @@ lemma g_parE [elim]:
   assumes "R,G \<turnstile> P { c\<^sub>1 || c\<^sub>2 } Q"
   obtains R\<^sub>1 G\<^sub>1 P\<^sub>1 Q\<^sub>1 R\<^sub>2 G\<^sub>2 P\<^sub>2 Q\<^sub>2 where 
     "R\<^sub>1,G\<^sub>1 \<turnstile> P\<^sub>1 { c\<^sub>1 } Q\<^sub>1" "R\<^sub>2,G\<^sub>2 \<turnstile> P\<^sub>2 { c\<^sub>2 } Q\<^sub>2"
-    "P \<subseteq> P\<^sub>1 \<inter> P\<^sub>2" "R \<subseteq> R\<^sub>1 \<inter> R\<^sub>2" "G\<^sub>1 \<union> G\<^sub>2 \<subseteq> G" "Q\<^sub>1 \<inter> Q\<^sub>2 \<subseteq> Q" "G\<^sub>1 \<subseteq> R\<^sub>2" "G\<^sub>2 \<subseteq> R\<^sub>1"
+    "P \<subseteq> left P\<^sub>1 \<inter> right P\<^sub>2" "R \<subseteq> R\<^sub>1 \<inter> R\<^sub>2" "G\<^sub>1 \<union> G\<^sub>2 \<subseteq> G" "left Q\<^sub>1 \<inter> right Q\<^sub>2 \<subseteq> Q" "G\<^sub>1 \<subseteq> R\<^sub>2" "G\<^sub>2 \<subseteq> R\<^sub>1"
   using assms
 proof (induct R G P "c\<^sub>1 || c\<^sub>2" Q)
   case (thread R G P Q)
-  then show ?case using parE by fast
+  then show ?case by blast
 next
   case (par R\<^sub>1 G\<^sub>1 P\<^sub>1 Q\<^sub>1 R\<^sub>2 G\<^sub>2 P\<^sub>2 Q\<^sub>2)
   show ?case using par(7)[OF par(1,3)] par(5,6) by blast
@@ -46,7 +44,7 @@ next
   proof (rule conseq(2), goal_cases)
     case (1 R\<^sub>1 G\<^sub>1 P\<^sub>1 Q\<^sub>1 R\<^sub>2 G\<^sub>2 P\<^sub>2 Q\<^sub>2)
     then show ?case using conseq(3,4,5,6) conseq(7)[OF 1(1,2)] by blast
-  qed  
+  qed (*  
 next
   case (frame R G P Q R' M)
   show ?case
@@ -55,13 +53,44 @@ next
     hence a: "R\<^sub>1 \<inter> R',G\<^sub>1 \<turnstile> P\<^sub>1 \<inter> M {c\<^sub>1} Q\<^sub>1 \<inter> M" "R\<^sub>2 \<inter> R',G\<^sub>2 \<turnstile> P\<^sub>2 \<inter> M {c\<^sub>2} Q\<^sub>2 \<inter> M"
       using rules.frame frame(3,4) by auto
     show ?case using 1(3,4,5,6,7,8) frame(4) frame(5)[OF a] by blast
-  qed
+  qed *)
 qed
+
+lemma leaf_mono[intro]:
+  "P \<subseteq> Q \<Longrightarrow> leaf P \<subseteq> leaf Q"
+  unfolding leaf_def by auto
+
+lemma left_mono[intro]:
+  "P \<subseteq> Q \<Longrightarrow> left P \<subseteq> left Q"
+  unfolding left_def by auto
+
+lemma right_mono[intro]:
+  "P \<subseteq> Q \<Longrightarrow> right P \<subseteq> right Q"
+  unfolding right_def by auto
+
+lemma leaf_stable[intro]:
+  "stable R P \<Longrightarrow> stable R (leaf P)"
+  unfolding leaf_def stable_def by auto
+
+lemma left_stable[intro]:
+  "stable R P \<Longrightarrow> stable R (left P)"
+  unfolding left_def stable_def by auto
+
+lemma right_stable[intro]:
+  "stable R P \<Longrightarrow> stable R (right P)"
+  unfolding right_def stable_def by auto
 
 lemma g_nilE [elim!]:
   assumes "R,G \<turnstile> P {Nil} Q"
   obtains M where "stable R M" "P \<subseteq> M" "M \<subseteq> Q"
-  using assms by (induct R G P "Nil :: ('a,'b) com" Q) blast+
+  using assms 
+proof (induct R G P "Nil :: ('a,'b,'c) com" Q)
+  case (thread R G P Q)
+  then show ?case using leaf_mono leaf_stable by blast 
+next
+  case (conseq R G P Q P' R' G' Q')
+  then show ?case by blast
+qed
 
 lemma g_stable_preE:
   assumes "R,G \<turnstile> P {c} Q"
@@ -69,15 +98,17 @@ lemma g_stable_preE:
   using assms 
 proof (induct)
   case (thread R G P c Q)
-  then show ?case using stable_preE by (metis rules.thread) 
-next
+  then show ?case using stable_preE by (metis rules.thread leaf_stable leaf_mono) 
+next 
   case (par R\<^sub>1 G\<^sub>1 P\<^sub>1 c\<^sub>1 Q\<^sub>1 R\<^sub>2 G\<^sub>2 P\<^sub>2 c\<^sub>2 Q\<^sub>2)
   show ?case
   proof (rule par(2), rule par(4), goal_cases)
     case (1 P1 P2)
-    hence "R\<^sub>1 \<inter> R\<^sub>2,G\<^sub>1 \<union> G\<^sub>2 \<turnstile> P1 \<inter> P2 {c\<^sub>1 || c\<^sub>2} Q\<^sub>1 \<inter> Q\<^sub>2"
+    hence "R\<^sub>1 \<inter> R\<^sub>2,G\<^sub>1 \<union> G\<^sub>2 \<turnstile> left P1 \<inter> right P2 {c\<^sub>1 || c\<^sub>2} left Q\<^sub>1 \<inter> right Q\<^sub>2"
       using rules.par par(5,6) by simp
-    thus ?case using par(7)[of "P1 \<inter> P2"] using 1 by auto
+    thus ?case using par(7)[of "left P1 \<inter> right P2"] 
+      using 1 left_stable right_stable right_mono left_mono 
+      by (metis inf_mono stable_conjI)
   qed 
 qed blast+
 
