Local_Rules.thy
@@ -14,12 +14,14 @@ begin
 section \<open>Base Rules\<close>
 
 text \<open>Rules of the logic over a thread, similar to standard Hoare-logic\<close>
-inductive lrules :: "'b rpred \<Rightarrow> 'b rpred \<Rightarrow> 'b pred \<Rightarrow> ('a,'b) com \<Rightarrow> 'b pred \<Rightarrow> bool" 
+inductive lrules :: "('b,'c) rpred \<Rightarrow> ('b,'c) rpred \<Rightarrow> ('b,'c) pred \<Rightarrow> ('a,'b,'c) com \<Rightarrow> ('b,'c) pred \<Rightarrow> bool" 
   ("_,_ \<turnstile>\<^sub>l _ {_} _" [20,0,0,0,20] 20)
 where
   nil[intro]:    "stable R P \<Longrightarrow> R,G \<turnstile>\<^sub>l P { Nil } P" |
   seq[intro]:    "R,G \<turnstile>\<^sub>l P { c\<^sub>1 } Q \<Longrightarrow> R,G \<turnstile>\<^sub>l Q { c\<^sub>2 } M \<Longrightarrow> R,G \<turnstile>\<^sub>l P { c\<^sub>1 ; c\<^sub>2 } M" |
+  ord[intro]:    "R,G \<turnstile>\<^sub>l P { c\<^sub>1 } Q \<Longrightarrow> R,G \<turnstile>\<^sub>l Q { c\<^sub>2 } M \<Longrightarrow> R,G \<turnstile>\<^sub>l P { c\<^sub>1 \<cdot> c\<^sub>2 } M" |
   choice[intro]: "R,G \<turnstile>\<^sub>l P { c\<^sub>1 } Q \<Longrightarrow> R,G \<turnstile>\<^sub>l P { c\<^sub>2 } Q \<Longrightarrow> R,G \<turnstile>\<^sub>l P { c\<^sub>1 \<sqinter> c\<^sub>2 } Q" |
+  bigchoice[intro]: "\<forall>s \<in> S. R,G \<turnstile>\<^sub>l P { seq2com s } Q \<Longrightarrow> R,G \<turnstile>\<^sub>l P { \<Sqinter> S } Q" |
   loop[intro]:   "stable R P \<Longrightarrow> R,G \<turnstile>\<^sub>l P { c } P \<Longrightarrow> R,G \<turnstile>\<^sub>l P { c* } P" |
   basic[intro]:  "R,G \<turnstile>\<^sub>A P {\<alpha>} Q \<Longrightarrow> R,G \<turnstile>\<^sub>l P { Basic \<alpha> } Q" |
   conseq[intro]: "R,G \<turnstile>\<^sub>l P { c } Q \<Longrightarrow> P' \<subseteq> P \<Longrightarrow> R' \<subseteq> R \<Longrightarrow> G \<subseteq> G' \<Longrightarrow> Q \<subseteq> Q' \<Longrightarrow> R',G' \<turnstile>\<^sub>l P' { c } Q'"
@@ -34,13 +36,13 @@ These mostly deal with complexities introduced by support conseq.
 lemma nilE [elim!]:
   assumes "R,G \<turnstile>\<^sub>l P {Nil} Q"
   obtains M where "stable R M" "P \<subseteq> M" "M \<subseteq> Q"
-  using assms by (induct R G P "Nil :: ('a,'b) com" Q) blast+
+  using assms by (induct R G P "Nil :: ('a,'b,'c) com" Q) blast+
 
 lemma basicE [elim!]:
   assumes "R,G \<turnstile>\<^sub>l P {Basic \<beta>} Q"
   obtains P' Q' where "P \<subseteq> P'" "R,G \<turnstile>\<^sub>A P' {\<beta>} Q'" "Q' \<subseteq> Q"
   using assms 
-proof (induct R G P "Basic \<beta> :: ('a,'b) com" Q)
+proof (induct R G P "Basic \<beta> :: ('a,'b,'c) com" Q)
   case (basic R G P Q)
   then show ?case by auto
 next
@@ -53,6 +55,12 @@ lemma seqE [elim]:
   obtains M  where "R,G \<turnstile>\<^sub>l P {c\<^sub>1} M" "R,G \<turnstile>\<^sub>l M {c\<^sub>2} Q"
   using assms 
   by (induct R G P "c\<^sub>1 ; c\<^sub>2" Q arbitrary: c\<^sub>1 c\<^sub>2) blast+
+
+lemma ordE [elim]:
+  assumes "R,G \<turnstile>\<^sub>l P {c\<^sub>1 \<cdot> c\<^sub>2} Q"
+  obtains M  where "R,G \<turnstile>\<^sub>l P {c\<^sub>1} M" "R,G \<turnstile>\<^sub>l M {c\<^sub>2} Q"
+  using assms 
+  by (induct R G P "c\<^sub>1 \<cdot> c\<^sub>2" Q arbitrary: c\<^sub>1 c\<^sub>2) blast+
 
 lemma choiceE [elim]:
   assumes "R,G \<turnstile>\<^sub>l P {c\<^sub>1 \<sqinter> c\<^sub>2} Q"
@@ -68,7 +76,7 @@ proof (induct R G P "c*" Q arbitrary: c)
   then show ?case by blast
 next
   case (conseq R G P Q P' R' G' Q')
-  then show ?case using lrules.conseq stable_conseqI by (metis subset_eq)
+  then show ?case using lrules.conseq stable_conseqI by (metis subset_iff)
 qed
 
 text \<open>No local judgement can be established over parallel composition or env steps\<close>
@@ -82,28 +90,52 @@ lemma parE [elim!]:
   obtains "False"
   using local_only assms by force
 
+lemma relE [elim!]:
+  assumes "R,G \<turnstile>\<^sub>l P { Rel r } Q"
+  obtains "False"
+  using local_only assms by force
+
 text \<open>Weaken the precondition of a judgement to a stable state\<close>
-lemma stable_preE:
+lemma stable_pre:
   assumes "R,G \<turnstile>\<^sub>l P {c} Q"
-  obtains P' where "P \<subseteq> P'" "stable R P'" "R,G \<turnstile>\<^sub>l P' {c} Q"
+  shows "\<exists>P'. P \<subseteq> P' \<and> stable R P' \<and> (R,G \<turnstile>\<^sub>l P' {c} Q)"
   using assms 
 proof (induct)
   case (basic R G P \<alpha> Q)
   then show ?case using atomic_rule_def by fast
 next
   case (choice R G P c\<^sub>1 Q c\<^sub>2)
-  show ?case
-  proof (rule choice(2), rule choice(4),  goal_cases)
-    case (1 P' P'')
-    have a: "stable R (P' \<inter> P'')" using 1 by auto
-    have b: "P \<subseteq> P' \<inter> P''" using 1 by auto
-    then show ?case using 1 choice(5)[OF b a] by blast
-  qed
+  then obtain P\<^sub>1 where 1: "P \<subseteq> P\<^sub>1" "stable R P\<^sub>1" "R,G \<turnstile>\<^sub>l P\<^sub>1 {c\<^sub>1} Q" by auto
+  then obtain P\<^sub>2 where 2: "P \<subseteq> P\<^sub>2" "stable R P\<^sub>2" "R,G \<turnstile>\<^sub>l P\<^sub>2 {c\<^sub>2} Q" using choice by auto
+  have "stable R (P\<^sub>1 \<inter> P\<^sub>2)" using 1 2 by auto
+  then show ?case using 1 2 by blast
+next
+  case (bigchoice S R G P Q)
+  hence "\<exists>P\<^sub>s. \<forall>s\<in>S. P \<subseteq> P\<^sub>s s \<and> stable R (P\<^sub>s s) \<and> (R,G \<turnstile>\<^sub>l P\<^sub>s s {seq2com s} Q)"
+    by metis
+  then obtain P\<^sub>s where s: "\<forall>s\<in>S. P \<subseteq> P\<^sub>s s \<and> stable R (P\<^sub>s s) \<and> (R,G \<turnstile>\<^sub>l P\<^sub>s s {seq2com s} Q)"
+    by blast
+  hence "stable R (\<Inter>s\<in>S. P\<^sub>s s)" by (auto simp: stable_def)
+  moreover have "P \<subseteq> (\<Inter>s\<in>S. P\<^sub>s s)" using s by auto
+  ultimately show ?case using s bigchoice.hyps(1) by blast
+next
+  case (conseq R G P c Q P' R' G' Q')
+  then show ?case by (meson lrules.conseq order_refl stable_conseqI subset_trans)
 qed blast+
 
-lemma [intro]:
-  "stable R {}"
-  by (auto simp: stable_def)
+lemma stable_preE:
+  assumes "R,G \<turnstile>\<^sub>l P {c} Q"
+  obtains P' where "P \<subseteq> P'" "stable R P'" "R,G \<turnstile>\<^sub>l P' {c} Q"
+  using assms stable_pre by metis
+
+lemma false_seqI:
+  assumes "\<forall>\<beta> \<in> set s. guar \<beta> G"
+  shows "R,G \<turnstile>\<^sub>l {} {seq2com s} {}"
+  using assms
+proof (induct s)
+  case (Cons a s)
+  then show ?case using atomic_rule_def by fastforce
+qed auto
 
 lemma falseI:
   assumes "\<forall>\<beta> \<in> basics c. guar \<beta> G" "local c"
@@ -112,6 +144,9 @@ lemma falseI:
 proof (induct c)
   case (Basic x)
   then show ?case using atomic_rule_def by force
+next
+  case (BigChoice S)
+  then show ?case using false_seqI by auto
 qed auto
 
 end
