Semantics.thy
@@ -10,11 +10,11 @@ Also introduces a notion of configuration, that couples programs and memory stat
 with transitions for the program and the environment.
 \<close>
 
-type_synonym ('a,'b) config = "('a,'b) com \<times> 'b"
+type_synonym ('a,'b,'c) config = "('a,'b,'c) com \<times> ('b \<times> 'c tree)"
 
 locale semantics = reordering fwd re + atomic vc beh
-  for vc :: "'a \<Rightarrow> 'b set"
-  and beh :: "'a \<Rightarrow> 'b rel"
+  for vc :: "'a \<Rightarrow> ('b \<times> 'c) set"
+  and beh :: "'a \<Rightarrow> ('b \<times> 'c) rel"
   and fwd :: "'a \<Rightarrow> 'a \<Rightarrow> 'a" ("_\<langle>_\<rangle>" [1000,0] 1000)
   and re :: "'a \<Rightarrow> 'a \<Rightarrow> bool" (infix "\<hookleftarrow>" 100)
 
@@ -25,27 +25,42 @@ section \<open>Program Transition Definitions\<close>
 
 text \<open>
 Semantics that collects reordering effects.
-Given c \<mapsto>[\<alpha>,r,\<alpha>'] c', this corresponds to c \<mapsto>\<alpha> c', such that
+Given c \<mapsto>[r,\<alpha>'] c', this corresponds to c \<mapsto>\<alpha><r> c', such that
 r should be the program \<alpha>' has to reorder with in c to execute and 
 \<alpha> should be \<alpha>' forwarded across r.\<close>
-inductive execute :: "('a,'b) com \<Rightarrow> 'a \<Rightarrow> ('a,'b) com \<Rightarrow> 'a \<Rightarrow> ('a,'b) com \<Rightarrow> bool"
-  ("_ \<mapsto>[_,_,_] _" [71,0,0,0,71] 70)
+inductive lcl_execute :: "('a,'b,'c) com \<Rightarrow> ('a,'b,'c) com \<Rightarrow> 'a \<Rightarrow> ('a,'b,'c) com \<Rightarrow> bool"
+  ("_ \<mapsto>[_,_] _" [71,0,0,71] 70)
   where
-  act[intro]:  "Basic \<alpha> \<mapsto>[\<alpha>,Nil,\<alpha>] Nil" |
-  seq[intro]:  "c\<^sub>1 \<mapsto>[\<alpha>,c,\<alpha>'] c\<^sub>1' \<Longrightarrow> c\<^sub>1 ; c\<^sub>2 \<mapsto>[\<alpha>,c,\<alpha>'] c\<^sub>1' ; c\<^sub>2" |
-  ooo[intro]:  "c\<^sub>1 \<mapsto>[\<alpha>,c,\<alpha>'] c\<^sub>1' \<Longrightarrow> \<gamma> < c\<^sub>2 <\<^sub>c \<alpha> \<Longrightarrow> c\<^sub>2 ; c\<^sub>1 \<mapsto>[\<gamma>,c\<^sub>2;c,\<alpha>'] c\<^sub>2 ; c\<^sub>1'" |
-  par1[intro]: "c\<^sub>1 \<mapsto>[\<alpha>,c,\<alpha>'] c\<^sub>1' \<Longrightarrow> c\<^sub>1 || c\<^sub>2 \<mapsto>[\<alpha>,c,\<alpha>'] c\<^sub>1' || c\<^sub>2" |
-  par2[intro]: "c\<^sub>2 \<mapsto>[\<alpha>,c,\<alpha>'] c\<^sub>2' \<Longrightarrow> c\<^sub>1 || c\<^sub>2 \<mapsto>[\<alpha>,c,\<alpha>'] c\<^sub>1 || c\<^sub>2'"
-inductive_cases execute[elim]: "c\<^sub>1 \<mapsto>[\<alpha>,c,\<alpha>'] c\<^sub>1'"
+  act[intro]: "Basic \<alpha> \<mapsto>[Nil,\<alpha>] Nil" |
+  seq[intro]: "c\<^sub>1 \<mapsto>[r,\<alpha>] c\<^sub>1' \<Longrightarrow> c\<^sub>1 ; c\<^sub>2 \<mapsto>[r,\<alpha>] c\<^sub>1' ; c\<^sub>2" |
+  ord[intro]: "c\<^sub>1 \<mapsto>[r,\<alpha>] c\<^sub>1' \<Longrightarrow> c\<^sub>1 \<cdot> c\<^sub>2 \<mapsto>[r,\<alpha>] c\<^sub>1' \<cdot> c\<^sub>2" |
+  ooo[intro]: "c\<^sub>1 \<mapsto>[r,\<alpha>] c\<^sub>1' \<Longrightarrow> \<alpha>' < c\<^sub>2 ; r <\<^sub>c \<alpha> \<Longrightarrow> c\<^sub>2 ; c\<^sub>1 \<mapsto>[c\<^sub>2 ; r ,\<alpha>] c\<^sub>2 ; c\<^sub>1'"
+inductive_cases lcl_execute[elim]: "c \<mapsto>[r,\<alpha>'] c'"
+
+text \<open>
+Semantics that collects reordering effects.
+Given c \<mapsto>[r,\<alpha>'] c', this corresponds to c \<mapsto>\<alpha><r> c', such that
+r should be the program \<alpha>' has to reorder with in c to execute and 
+\<alpha> should be \<alpha>' forwarded across r.\<close>
+inductive glb_execute :: "('a,'b,'c) com \<Rightarrow> ('b \<times> 'c tree) rel \<Rightarrow> ('a,'b,'c) com \<Rightarrow> bool"
+  ("_ \<mapsto>[_] _" [71,0,71] 70)
+  where
+  lcl[intro]: "c \<mapsto>[r,\<alpha>] c' \<Longrightarrow> c \<mapsto>[leaf\<^sub>r (eval \<alpha>\<llangle>r\<rrangle>)] c'" |
+  par1[intro]: "c\<^sub>1 \<mapsto>[g] c\<^sub>1' \<Longrightarrow> c\<^sub>1 || c\<^sub>2 \<mapsto>[left\<^sub>r g] c\<^sub>1' || c\<^sub>2" |
+  par2[intro]: "c\<^sub>2 \<mapsto>[g] c\<^sub>2' \<Longrightarrow> c\<^sub>1 || c\<^sub>2 \<mapsto>[right\<^sub>r g] c\<^sub>1 || c\<^sub>2'"
+inductive_cases glb_execute[elim]: "c \<mapsto>[g] c'"
 
 text \<open>Small step semantics for a silent step\<close>
-inductive silent :: "('a,'b) com \<Rightarrow> ('a,'b) com \<Rightarrow> bool"
+inductive silent :: "('a,'b,'c) com \<Rightarrow> ('a,'b,'c) com \<Rightarrow> bool"
   ("_ \<leadsto> _" [71,71] 70)
   where
   seq1[intro]:  "c\<^sub>1 \<leadsto> c\<^sub>1' \<Longrightarrow> c\<^sub>1 ; c\<^sub>2 \<leadsto> c\<^sub>1' ; c\<^sub>2" |
+  ord1[intro]:  "c\<^sub>1 \<leadsto> c\<^sub>1' \<Longrightarrow> c\<^sub>1 \<cdot> c\<^sub>2 \<leadsto> c\<^sub>1' \<cdot> c\<^sub>2" |
   seq2[intro]:  "c\<^sub>2 \<leadsto> c\<^sub>2' \<Longrightarrow> c\<^sub>1 ; c\<^sub>2 \<leadsto> c\<^sub>1 ; c\<^sub>2'" |
   seqE1[intro]: "Nil ; c\<^sub>1 \<leadsto> c\<^sub>1" |
   seqE2[intro]: "c\<^sub>1 ; Nil \<leadsto> c\<^sub>1" |
+  ordE[intro]:  "Nil \<cdot> c\<^sub>1 \<leadsto> c\<^sub>1" |
+  bigc[intro]:  "s \<in> S \<Longrightarrow> (\<Sqinter> S) \<leadsto> seq2com s" |
   left[intro]:  "c\<^sub>1 \<sqinter> c\<^sub>2 \<leadsto> c\<^sub>1" |
   right[intro]: "c\<^sub>1 \<sqinter> c\<^sub>2 \<leadsto> c\<^sub>2" |
   loop1[intro]: "c* \<leadsto> Nil" |
@@ -58,13 +73,26 @@ inductive_cases silentE[elim]: "c\<^sub>1 \<leadsto> c\<^sub>1'"
 
 text \<open>An execution step implies the program has changed\<close>
 lemma execute_neq:
-  assumes "c \<mapsto>[\<alpha>,r,\<alpha>'] c'"
+  assumes "c \<mapsto>[r,\<alpha>'] c'"
   shows "c \<noteq> c'"
   using assms by (induct) auto
 
 lemma [simp]:
-  "c \<mapsto>[\<alpha>,r,\<alpha>'] c = False"
+  "c \<mapsto>[r,\<alpha>'] c = False"
   using execute_neq by blast
+
+lemma gexecute_neq:
+  assumes "c \<mapsto>[g] c'"
+  shows "c \<noteq> c'"
+  using assms by (induct) auto
+
+lemma [simp]:
+  "c \<mapsto>[g] c = False"
+  using gexecute_neq by blast
+
+lemma [intro]:
+  "local (seq2com s)"
+  by (induct s) auto
 
 text \<open>A silent step will not introduce parallelism\<close>
 lemma local_silent:
@@ -73,37 +101,31 @@ lemma local_silent:
 
 text \<open>An execution step will not introduce parallelism\<close>
 lemma local_execute:
-  "c \<mapsto>[\<alpha>,r,\<alpha>'] c' \<Longrightarrow> local c \<Longrightarrow> local c'"
-  by (induct rule: execute.induct) auto
-
-text \<open>Instrumented semantics collects valid reorderings\<close>
-lemma collect_reorder:
-  assumes "c \<mapsto>[\<alpha>',r,\<alpha>] c'"
-  shows "\<alpha>' < r <\<^sub>c \<alpha>"
-  using assms by (induct, auto)
+  "c \<mapsto>[r,\<alpha>'] c' \<Longrightarrow> local c \<Longrightarrow> local c'"
+  by (induct rule: lcl_execute.induct) auto
 
 section \<open>Transition Definitions\<close>
 
 text \<open>These transitions are over configurations of (program,state)\<close>
 
 text \<open>Environment Transition\<close>
-abbreviation env_tran :: "('a,'b) config \<Rightarrow> ('a,'b) config \<Rightarrow> bool" ("_ -e\<rightarrow> _" [81,81] 80)
+abbreviation env_tran :: "('a,'b,'c) config \<Rightarrow> ('a,'b,'c) config \<Rightarrow> bool" ("_ -e\<rightarrow> _" [81,81] 80)
   where "s -e\<rightarrow> s' \<equiv> fst s = fst s'"
 
 text \<open>Program Execution Transition\<close>
-abbreviation exec_tran :: "('a,'b) config \<Rightarrow> ('a,'b) config \<Rightarrow> bool" ("_ -\<alpha>\<rightarrow> _" [81,81] 80)
-  where "s -\<alpha>\<rightarrow> s' \<equiv> \<exists>\<alpha> r \<alpha>'. fst s \<mapsto>[\<alpha>,r,\<alpha>'] (fst s') \<and> (snd s,snd s') \<in> eval \<alpha>"
+abbreviation exec_tran :: "('a,'b,'c) config \<Rightarrow> ('a,'b,'c) config \<Rightarrow> bool" ("_ -\<alpha>\<rightarrow> _" [81,81] 80)
+  where "s -\<alpha>\<rightarrow> s' \<equiv> \<exists>g. fst s \<mapsto>[g] (fst s') \<and> (snd s,snd s') \<in> g"
 
 text \<open>Program Silent Transition\<close>
-abbreviation sil_tran :: "('a,'b) config \<Rightarrow> ('a,'b) config \<Rightarrow> bool" ("_ -s\<rightarrow> _" [81,81] 80)
+abbreviation sil_tran :: "('a,'b,'c) config \<Rightarrow> ('a,'b,'c) config \<Rightarrow> bool" ("_ -s\<rightarrow> _" [81,81] 80)
   where "s -s\<rightarrow> s' \<equiv> fst s \<leadsto> fst s' \<and> snd s = snd s'"
 
 text \<open>Program Transition\<close>
-abbreviation com_tran :: "('a,'b) config \<Rightarrow> ('a,'b) config \<Rightarrow> bool" ("_ -c\<rightarrow> _" [81,81] 80)
+abbreviation com_tran :: "('a,'b,'c) config \<Rightarrow> ('a,'b,'c) config \<Rightarrow> bool" ("_ -c\<rightarrow> _" [81,81] 80)
   where "s -c\<rightarrow> s' \<equiv> s -\<alpha>\<rightarrow> s' \<or> s -s\<rightarrow> s'"
 
 text \<open>Collect of all possible transitions\<close>
-inductive_set transitions :: "('a,'b) config list set"
+inductive_set transitions :: "('a,'b,'c) config list set"
   where 
     one[intro]: "[s] \<in> transitions" |
     env[intro]: "s -e\<rightarrow> s' \<Longrightarrow> s'#t \<in> transitions \<Longrightarrow> s#s'#t \<in> transitions" |
