Soundness.thy
@@ -13,17 +13,17 @@ section \<open>Helper Definitions\<close>
 
 text \<open>Strongest postcondition across arbitrary environment steps, 
       used to compute some new intermediate states for reasoning\<close>
-definition sp :: "'a \<Rightarrow> 'b rpred \<Rightarrow> 'b pred \<Rightarrow> 'b pred"
-  where "sp \<alpha> R P \<equiv> {m. \<exists>m' m''. m' \<in> P \<and> (m',m'') \<in> beh \<alpha> \<and> (m'',m) \<in> R\<^sup>* }"
+definition sp :: "'a \<Rightarrow> ('b,'c) rpred \<Rightarrow> ('b,'c) pred \<Rightarrow> ('b,'c) pred"
+  where "sp \<alpha> R P \<equiv> {m. \<exists>m' m''. m' \<in> P \<and> (m',m'') \<in> beh \<alpha> \<and> (m'',m) \<in> fullR (R\<^sup>* ) }"
 
 text \<open>Re-establish an atomic judgement with its strongest postcondition\<close>
 lemma atomic_strongest:
   assumes "R,G \<turnstile>\<^sub>A P {\<alpha>} Q"
   shows "R,G \<turnstile>\<^sub>A P {\<alpha>} sp \<alpha> R P \<and> sp \<alpha> R P \<subseteq> Q"
 proof -
-  have "Q \<subseteq> {m. \<forall>m'. (m,m') \<in> R\<^sup>* \<longrightarrow> m' \<in> Q}" "P \<subseteq> wp\<^sub>\<alpha> \<alpha> Q" 
+  have "Q \<subseteq> {m. \<forall>m'. (m,m') \<in> fullR (R\<^sup>* ) \<longrightarrow> m' \<in> Q}" "P \<subseteq> wp\<^sub>\<alpha> \<alpha> Q" 
     using assms stable_transitive unfolding atomic_rule_def wp_def by fast+
-  hence "sp \<alpha> R P \<subseteq> Q" by (auto simp: sp_def wp_def)
+  hence "sp \<alpha> R P \<subseteq> Q" apply (auto simp: sp_def wp_def) by blast
   moreover have "R,G \<turnstile>\<^sub>A P {\<alpha>} (sp \<alpha> R P)"
     using assms unfolding atomic_rule_def wp_def stable_def sp_def by fastforce
   ultimately show ?thesis by auto
@@ -36,7 +36,7 @@ text \<open>
   The precondition P and postcondition Q are preserved.
 \<close>
 lemma reorder_action:
-  assumes "R,G \<turnstile>\<^sub>A P {\<beta>} M" "R,G \<turnstile>\<^sub>A M {\<alpha>} Q" "\<beta> \<hookleftarrow> \<alpha>\<langle>\<beta>\<rangle>" "inter\<^sub>\<alpha> R G \<beta> \<alpha>"
+  assumes "R,G \<turnstile>\<^sub>A P {\<beta>} M" "R,G \<turnstile>\<^sub>A M {\<alpha>} Q" "inter\<^sub>\<alpha> R G \<beta> \<alpha>"
   obtains M' where "R,G \<turnstile>\<^sub>A P {\<alpha>\<langle>\<beta>\<rangle>} M'" "R,G \<turnstile>\<^sub>A M' {\<beta>} Q"
 proof -
   \<comment> \<open>Nominate the strongest-postcondition of \<alpha> from P as the state between \<alpha> and \<beta>\<close>
@@ -49,26 +49,26 @@ proof -
 
   \<comment> \<open>Extract order independence properties\<close> 
   have ref: "Env R ; Basic \<beta> ; Env R ; Basic \<alpha> \<sqsubseteq> Env R ; Basic \<alpha>\<langle>\<beta>\<rangle> ; Env R ; Basic \<beta>"
-    using assms(4) by (auto simp: inter\<^sub>\<alpha>_def)
-  have g: "guar \<alpha>\<langle>\<beta>\<rangle> G" using assms(4) by (auto simp: inter\<^sub>\<alpha>_def)
+    using assms(3) by (auto simp: inter\<^sub>\<alpha>_def)
+  have g: "guar \<alpha>\<langle>\<beta>\<rangle> G" using assms(3) by (auto simp: inter\<^sub>\<alpha>_def)
 
   \<comment> \<open>Show transition from P to Q is independent of order\<close>
-  have p: "P \<subseteq> wp\<^sub>\<alpha> \<beta> M" "M \<subseteq> wp\<^sub>\<alpha> \<alpha> Q" "M \<subseteq> wp UNIV (R\<^sup>* ) M" "P \<subseteq>  wp UNIV (R\<^sup>* ) P" "Q \<subseteq>  wp UNIV (R\<^sup>* ) Q"
+  have p: "P \<subseteq> wp\<^sub>\<alpha> \<beta> M" "M \<subseteq> wp\<^sub>\<alpha> \<alpha> Q" "M \<subseteq> wp UNIV (fullR (R\<^sup>* )) M" "P \<subseteq>  wp UNIV (fullR (R\<^sup>* )) P" "Q \<subseteq>  wp UNIV (fullR (R\<^sup>* )) Q"
     using assms(1,2)  unfolding atomic_rule_def by (auto intro!: stable_wp\<^sub>tI)
-  hence "P \<subseteq>  wp UNIV (R\<^sup>* ) (wp\<^sub>\<alpha> \<beta> ( wp UNIV (R\<^sup>* ) (wp\<^sub>\<alpha> \<alpha> Q)))" unfolding wp_def by blast
-  hence exec: "P \<subseteq>  wp UNIV (R\<^sup>* ) (wp\<^sub>\<alpha> \<alpha>\<langle>\<beta>\<rangle> ( wp UNIV (R\<^sup>* ) (wp\<^sub>\<alpha> \<beta> Q)))" using ref by (auto simp: refine_def)
+  hence "P \<subseteq>  wp UNIV (fullR (R\<^sup>* )) (wp\<^sub>\<alpha> \<beta> ( wp UNIV (fullR (R\<^sup>* )) (wp\<^sub>\<alpha> \<alpha> Q)))" unfolding wp_def by force
+  hence exec: "P \<subseteq>  wp UNIV (fullR (R\<^sup>* )) (wp\<^sub>\<alpha> \<alpha>\<langle>\<beta>\<rangle> ( wp UNIV (fullR (R\<^sup>* )) (wp\<^sub>\<alpha> \<beta> Q)))" using ref by (auto simp: refine_def)
   hence vc: "P \<subseteq> vc \<alpha>\<langle>\<beta>\<rangle>" by (auto simp: wp_def)
 
   \<comment> \<open>Establish the late judgement over \<beta>\<close>
   have "R,G \<turnstile>\<^sub>A ?M {\<beta>} Q" 
   proof (unfold atomic_rule_def, intro conjI Int_greatest)
-    show "?M \<subseteq> wp\<^sub>\<alpha> \<beta> Q" using exec unfolding wp_def sp_def by blast
+    show "?M \<subseteq> wp\<^sub>\<alpha> \<beta> Q" using exec unfolding wp_def sp_def by fast
   qed (insert stablePQ stableM, auto)
 
   \<comment> \<open>Establish the early judgement over the new \<alpha>\<close>
   moreover have "R,G \<turnstile>\<^sub>A P {\<alpha>\<langle>\<beta>\<rangle>} ?M"
   proof (unfold atomic_rule_def, intro conjI Int_greatest)
-    show "P \<subseteq> wp\<^sub>\<alpha> \<alpha>\<langle>\<beta>\<rangle> ?M" using vc unfolding wp_def wf_def sp_def by blast
+    show "P \<subseteq> wp\<^sub>\<alpha> \<alpha>\<langle>\<beta>\<rangle> ?M" using vc unfolding wp_def wf_def sp_def by fast
   qed (insert stablePQ stableM g, auto)
 
   ultimately show ?thesis using that by blast
@@ -79,76 +79,49 @@ text \<open>
   interference property.
 \<close>
 lemma reorder_prog:
-  assumes "R,G \<turnstile>\<^sub>l P {c} M" "R,G \<turnstile>\<^sub>A M {\<alpha>} Q" "\<alpha>' < c <\<^sub>c \<alpha>" "inter\<^sub>c R G c \<alpha>"
-  obtains M' P' where "P \<subseteq> P'" "R,G \<turnstile>\<^sub>A P' {\<alpha>'} M'" "R,G \<turnstile>\<^sub>l M' {c} Q"
+  assumes "R,G \<turnstile>\<^sub>l P {c} M" "R,G \<turnstile>\<^sub>A M {\<alpha>} Q" "inter\<^sub>c R G c \<alpha>"
+  obtains M' P' where "P \<subseteq> P'" "R,G \<turnstile>\<^sub>A P' {\<alpha>\<llangle>c\<rrangle>} M'" "R,G \<turnstile>\<^sub>l M' {c} Q"
   using assms
-proof (induct c arbitrary: R G P M Q \<alpha>' \<alpha>)
+proof (induct c arbitrary: R G P M Q \<alpha>)
   case Nil
   hence "P \<subseteq> M" by blast
   then show ?case using Nil by (auto simp: atomic_rule_def)
 next
   case (Basic \<beta>)
-  have \<alpha>: "\<beta> \<hookleftarrow> \<alpha>\<langle>\<beta>\<rangle>" "\<alpha>' = \<alpha>\<langle>\<beta>\<rangle>" using Basic by auto
   obtain P' N' where \<beta>: "P \<subseteq> P'" "R,G \<turnstile>\<^sub>A P' {\<beta>} N'" "N' \<subseteq> M" using Basic by auto
   have m': "R,G \<turnstile>\<^sub>A N' {\<alpha>} Q"
     using atomic_pre[OF Basic(3)] \<beta>(2,3) Basic(3) by (auto simp: atomic_rule_def)
   obtain M' where m'': "R,G \<turnstile>\<^sub>A P' {\<alpha>\<langle>\<beta>\<rangle>} M'" "R,G \<turnstile>\<^sub>A M' {\<beta>} Q"
-    using reorder_action[OF \<beta>(2) m'(1) \<alpha>(1)] Basic by auto
+    using reorder_action[OF \<beta>(2) m'(1)] Basic by auto
   have "R,G \<turnstile>\<^sub>l M' {Basic \<beta>} Q" by (rule lrules.basic[OF m''(2)])
-  then show ?case using Basic(1) \<beta>(1) m''(1) \<alpha>(2) by auto
+  then show ?case using Basic(1) \<beta>(1) m''(1) by auto
 next
   case (Seq c\<^sub>1 c\<^sub>2)
-  obtain \<alpha>\<^sub>n where \<alpha>: "\<alpha>' < c\<^sub>1 <\<^sub>c \<alpha>\<^sub>n" "\<alpha>\<^sub>n < c\<^sub>2 <\<^sub>c \<alpha>" using Seq by auto
   obtain M' where m: "R,G \<turnstile>\<^sub>l P {c\<^sub>1} M'" "R,G \<turnstile>\<^sub>l M' {c\<^sub>2} M" using Seq(4) by fast
-  have i: "inter\<^sub>c R G c\<^sub>1 \<alpha>\<^sub>n" "inter\<^sub>c R G c\<^sub>2 \<alpha>" using Seq \<alpha> by auto
+  have i: "inter\<^sub>c R G c\<^sub>1 \<alpha>\<llangle>c\<^sub>2\<rrangle>" "inter\<^sub>c R G c\<^sub>2 \<alpha>" using Seq by auto
   show ?case
-  proof (rule Seq(2)[OF _ m(2) Seq(5) \<alpha>(2) i(2)], goal_cases outer)
+  proof (rule Seq(2)[OF _ m(2) Seq(5) i(2)], goal_cases outer)
     case (outer P' N')
     hence c1: "R,G \<turnstile>\<^sub>l P {c\<^sub>1} P'" using m(1) conseq by auto
     show ?case 
-    proof (rule Seq(1)[OF _ c1 outer(2) \<alpha>(1) i(1)], goal_cases inner)
+    proof (rule Seq(1)[OF _ c1 outer(2) i(1)], goal_cases inner)
       case (inner P'' M'')
       then show ?case using Seq(3) outer by auto
     qed
   qed
 next
-  case (Choice c\<^sub>1 c\<^sub>2)
-  hence \<alpha>: "\<alpha>' < c\<^sub>1 <\<^sub>c \<alpha>" "\<alpha>' < c\<^sub>2 <\<^sub>c \<alpha>" by auto
-  obtain m: "R,G \<turnstile>\<^sub>l P {c\<^sub>1} M" "R,G \<turnstile>\<^sub>l P {c\<^sub>2} M" using Choice(4) by blast
-  have i: "inter\<^sub>c R G c\<^sub>1 \<alpha>" "inter\<^sub>c R G c\<^sub>2 \<alpha>" using Choice by auto
+  case (Ord c\<^sub>1 c\<^sub>2)
+  obtain M' where m: "R,G \<turnstile>\<^sub>l P {c\<^sub>1} M'" "R,G \<turnstile>\<^sub>l M' {c\<^sub>2} M" using Ord(4) by fast
+  have i: "inter\<^sub>c R G c\<^sub>1 \<alpha>\<llangle>c\<^sub>2\<rrangle>" "inter\<^sub>c R G c\<^sub>2 \<alpha>" using Ord by auto
   show ?case
-  proof (rule Choice(2)[OF _ m(2) Choice(5) \<alpha>(2) i(2)], goal_cases outer)
+  proof (rule Ord(2)[OF _ m(2) Ord(5) i(2)], goal_cases outer)
     case (outer P' N')
+    hence c1: "R,G \<turnstile>\<^sub>l P {c\<^sub>1} P'" using m(1) conseq by auto
     show ?case 
-    proof (rule Choice(1)[OF _ m(1) Choice(5) \<alpha>(1) i (1)], goal_cases inner)
-      case (inner P'' N'')
-      hence "R,G \<turnstile>\<^sub>l (N' \<inter> N'') {c\<^sub>1} Q"
-        using outer by (meson Int_lower2 subset_refl lrules.conseq)
-      moreover have "R,G \<turnstile>\<^sub>l (N' \<inter> N'') {c\<^sub>2} Q" 
-        using inner outer by (meson Int_lower1 subset_refl lrules.conseq)
-      ultimately have "R,G \<turnstile>\<^sub>l (N' \<inter> N'') {c\<^sub>1 \<sqinter> c\<^sub>2} Q" by auto
-      moreover have "P \<subseteq> P' \<inter> P''" using outer inner by auto
-      ultimately show ?case using actomic_conjI[OF outer(2) inner(2)] Choice(3) by blast 
+    proof (rule Ord(1)[OF _ c1 outer(2) i(1)], goal_cases inner)
+      case (inner P'' M'')
+      then show ?case using Ord(3) outer by auto
     qed
-  qed
-next
-  case (Loop c)
-  then obtain I where i: "P \<subseteq> I" "R,G \<turnstile>\<^sub>l I {c} I" "stable R I" "I \<subseteq> M" by auto
-  have [simp]: "\<alpha>' = \<alpha>" using Loop by auto
-  have \<alpha>: "\<alpha> < c <\<^sub>c \<alpha>" using Loop by auto
-  have "R,G \<turnstile>\<^sub>A I {\<alpha>} Q" using Loop(4) i(3,4) by (meson atomic_pre)
-  hence s: "R,G \<turnstile>\<^sub>A I {\<alpha>} (sp \<alpha> R I)" "sp \<alpha> R I \<subseteq> Q" using atomic_strongest by blast+
-  have d: "inter\<^sub>c R G c \<alpha>" using Loop by auto
-
-  show ?case
-  proof (rule Loop(1)[OF _ i(2) s(1) \<alpha> d], goal_cases outer)
-    case (outer P' I')
-    hence "R,G \<turnstile>\<^sub>A I {\<alpha>} I'" using i(3) by (meson atomic_pre)
-    hence "sp \<alpha> R I \<subseteq> I'" using atomic_strongest by blast
-    hence "R,G \<turnstile>\<^sub>l (sp \<alpha> R I) {c} (sp \<alpha> R I)" using outer(3) lrules.conseq by auto
-    hence "R,G \<turnstile>\<^sub>l (sp \<alpha> R I) {c*} (sp \<alpha> R I)" using s(1) by (meson loop atomic_rule_def)
-    hence "R,G \<turnstile>\<^sub>l (sp \<alpha> R I) {c*} Q" using s(2) conseq by blast
-    then show ?case using Loop(2)[OF i(1)] s(1) by simp
   qed
 qed auto
 
@@ -164,6 +137,9 @@ proof (induct arbitrary: c' rule: lrules.induct)
   case (seq R G P c\<^sub>1 Q c\<^sub>2 M)
   show ?case using seq(5,1,2,3,4) by cases blast+
 next
+  case (ord R G P c\<^sub>1 Q c\<^sub>2 M)
+  show ?case using ord(5,1,2,3,4) by cases blast+
+next
   case (loop R P G c)
   thus ?case by cases blast+
 qed auto
@@ -176,109 +152,186 @@ lemma g_rewriteI [intro]:
   using assms
 proof (induct arbitrary: c' rule: rules.induct)
   case (par R\<^sub>1 G\<^sub>1 P\<^sub>1 c\<^sub>1 Q\<^sub>1 R\<^sub>2 G\<^sub>2 P\<^sub>2 c\<^sub>2 Q\<^sub>2)
-  show ?case using par(7,1,2,3,4,5,6) by (cases) blast+
+  show ?case using par(7,1,2,3,4,5,6)
+    apply cases
+    apply blast
+    apply blast
+    apply clarsimp
+    sorry
 qed auto
 
 text \<open>Local judgements are preserved across reordered interference-free execution steps\<close>
 lemma stepI:
-  assumes "c \<mapsto>[\<alpha>,r,\<alpha>'] c'" "R,G \<turnstile>\<^sub>l P {c} Q"
-  assumes "inter\<^sub>c R G r \<alpha>'"
-  shows "\<exists>P' M. P \<subseteq> P' \<and> (R,G \<turnstile>\<^sub>A P' {\<alpha>} M) \<and> (R,G \<turnstile>\<^sub>l M {c'} Q)"
+  assumes "c \<mapsto>[r,\<alpha>] c'" "R,G \<turnstile>\<^sub>l P {c} Q"
+  assumes "inter\<^sub>c R G r \<alpha>"
+  shows "\<exists>P' M. P \<subseteq> P' \<and> (R,G \<turnstile>\<^sub>A P' {\<alpha>\<llangle>r\<rrangle>} M) \<and> (R,G \<turnstile>\<^sub>l M {c'} Q)"
   using assms
 proof (induct arbitrary: P R G Q)
   case (act \<alpha>)
-  then show ?case by (elim basicE) (meson atomic_rule_def nil lrules.conseq order_refl)
+  then show ?case
+    apply (elim basicE)
+    apply simp
+    apply (meson atomic_rule_def nil lrules.conseq order_refl)
+    done
 next
-  case (seq c\<^sub>1 \<alpha> c \<alpha>' c\<^sub>1' c\<^sub>2)
+  case (seq c\<^sub>1 c \<alpha>' c\<^sub>1' c\<^sub>2)
   obtain M' where m: "R,G \<turnstile>\<^sub>l P {c\<^sub>1} M'" "R,G \<turnstile>\<^sub>l M' {c\<^sub>2} Q" using seq by fast
   then show ?case using seq(2)[OF m(1) seq(4)] m(2) by blast
 next
-  case (ooo c\<^sub>2 \<alpha> c \<alpha>' c\<^sub>2' \<gamma> c\<^sub>1)
-  obtain M' where m: "R,G \<turnstile>\<^sub>l P {c\<^sub>1} M'" "R,G \<turnstile>\<^sub>l M' {c\<^sub>2} Q" using ooo by fast
-  have i: "inter\<^sub>c R G c\<^sub>1 (\<alpha>'\<llangle>c\<rrangle>)" "inter\<^sub>c R G c \<alpha>'" using ooo by auto
-  obtain P' M where m': "M' \<subseteq> P'" "R,G \<turnstile>\<^sub>A P' {\<alpha>} M" "R,G \<turnstile>\<^sub>l M {c\<^sub>2'} Q"
+  case (ooo c\<^sub>2 c \<alpha> c\<^sub>2' \<alpha>' c\<^sub>1)
+  obtain M' where m: "R,G \<turnstile>\<^sub>l P {c\<^sub>1} M'" "R,G \<turnstile>\<^sub>l M' {c\<^sub>2} Q" using ooo(4) by blast
+  have i: "inter\<^sub>c R G c\<^sub>1 (\<alpha>\<llangle>c\<rrangle>)" "inter\<^sub>c R G c \<alpha>" using ooo by auto
+  obtain P' M where m': "M' \<subseteq> P'" "R,G \<turnstile>\<^sub>A P' {\<alpha>\<llangle>c\<rrangle>} M" "R,G \<turnstile>\<^sub>l M {c\<^sub>2'} Q"
     using ooo(2)[OF m(2) i(2)] by blast
   hence m'': "R,G \<turnstile>\<^sub>l P {c\<^sub>1} P'" using m(1) by blast
-  have "\<alpha>'\<llangle>c\<rrangle> = \<alpha>" using ooo(1) collect_reorder by auto
-  then show ?case using reorder_prog[OF m'' m'(2) ooo(3)] i(1) m'(3) by (metis lrules.seq)
-qed auto
+  then show ?case using reorder_prog[OF m'' m'(2)] i(1) m'(3) by simp (metis lrules.seq)
+next
+  case (ord c\<^sub>1 c \<alpha> c\<^sub>1' c\<^sub>2)
+  obtain M' where m: "R,G \<turnstile>\<^sub>l P {c\<^sub>1} M'" "R,G \<turnstile>\<^sub>l M' {c\<^sub>2} Q" using ord by fast
+  then show ?case using ord(2)[OF m(1) ord(4)] m(2) by blast
+qed 
+
+abbreviation fullG
+  where "fullG G \<equiv> {((g,l),(g',l')). (g,g') \<in> G}"
+
+lemma gexec_localE:
+  assumes "c \<mapsto>[g] c'" "local c"
+  obtains \<alpha> r where "c \<mapsto>[r,\<alpha>] c'" "g = leaf\<^sub>r (eval \<alpha>\<llangle>r\<rrangle>)"
+  using assms
+  by (induct) auto
 
 text \<open>Global judgements are preserved across execution steps - reordering or not \<close>
 lemma g_stepI:
   assumes "R,G \<turnstile> P {c} Q"
-  assumes "c \<mapsto>[\<alpha>,r,\<alpha>'] c'"
-  shows "\<exists>P' M. P \<subseteq> P' \<and> (R,G \<turnstile>\<^sub>A P' {\<alpha>} M) \<and> (R,G \<turnstile> M {c'} Q)"
+  assumes "c \<mapsto>[g] c'"
+  shows "\<exists>M v. P \<subseteq> wp v g M \<and> ({m. fst m \<in> v} \<inter> g) \<subseteq> fullG (G\<^sup>=) \<and> (R,G \<turnstile> M {c'} Q)"
   using assms
-proof (induct arbitrary: \<alpha> c' rule: rules.induct)
+proof (induct arbitrary: g c' rule: rules.induct)
   case (par R\<^sub>1 G\<^sub>1 P\<^sub>1 c\<^sub>1 Q\<^sub>1 R\<^sub>2 G\<^sub>2 P\<^sub>2 c\<^sub>2 Q\<^sub>2)
   show ?case using par(7)
   proof cases
-    case (par1 c\<^sub>1')
+    case (lcl r \<alpha>)
+    then show ?thesis by auto
+  next
+    case (par1 g' c\<^sub>1')
     obtain M\<^sub>2 where m2: "P\<^sub>2 \<subseteq> M\<^sub>2" "stable R\<^sub>2 M\<^sub>2" "R\<^sub>2,G\<^sub>2 \<turnstile> M\<^sub>2 {c\<^sub>2} Q\<^sub>2" using par
       by (meson g_stable_preE)
-    obtain P M\<^sub>1 where m1: "P\<^sub>1 \<subseteq> P" "R\<^sub>1,G\<^sub>1 \<turnstile>\<^sub>A P { \<alpha> } M\<^sub>1" "R\<^sub>1,G\<^sub>1 \<turnstile> M\<^sub>1 {c\<^sub>1'} Q\<^sub>1" 
-      using par1 par(2)[OF par1(2)] by blast
-    hence "R\<^sub>1 \<inter> R\<^sub>2,G\<^sub>1 \<union> G\<^sub>2 \<turnstile> M\<^sub>1 \<inter> M\<^sub>2 {c'} Q\<^sub>1 \<inter> Q\<^sub>2" using par1 m2 par by blast
-    moreover have "R\<^sub>1 \<inter> R\<^sub>2,G\<^sub>1 \<union> G\<^sub>2 \<turnstile>\<^sub>A P \<inter> M\<^sub>2 { \<alpha> } M\<^sub>1 \<inter> M\<^sub>2" 
-      using m1(2) m2(2) par.hyps(6) by blast
-    ultimately show ?thesis using m2(1) m1(1) by blast
+    obtain M\<^sub>1 v where m1: "P\<^sub>1 \<subseteq> wp v g' M\<^sub>1" "({m. fst m \<in> v} \<inter> g') \<subseteq> fullG (G\<^sub>1\<^sup>=)" "R\<^sub>1,G\<^sub>1 \<turnstile> M\<^sub>1 {c\<^sub>1'} Q\<^sub>1"
+      using par1 par(2)[OF par1(3)] by blast
+    hence "R\<^sub>1 \<inter> R\<^sub>2,G\<^sub>1 \<union> G\<^sub>2 \<turnstile> left M\<^sub>1 \<inter> right M\<^sub>2 {c'} left Q\<^sub>1 \<inter> right Q\<^sub>2" 
+      using par1 m2 par by blast
+    moreover have "left P\<^sub>1 \<inter> right P\<^sub>2 \<subseteq> wp (left v) g (left M\<^sub>1 \<inter> right M\<^sub>2)" 
+      using par1 m2(1,2) m1(1,2) par.hyps(6)
+      unfolding left_def right_def left\<^sub>r_def wp_def stable_def
+      apply auto
+      apply (subgoal_tac "((gb, lb), g'a, l') \<in> fullG (R\<^sub>2\<^sup>=)")
+      apply (subgoal_tac "(gb, rb) \<in> M\<^sub>2")
+      apply auto
+      apply (subgoal_tac "((gb, lb), g'a, l') \<in> {((g, l), g', l').
+           (g, g') \<in> G\<^sub>1 \<or> g = g'}")
+      apply auto
+      apply (subgoal_tac "((gb, lb), g'a, l') \<in> {m. fst m \<in> v} \<inter> g'")
+      apply blast
+      by auto
+    moreover have "({m. fst m \<in> (left v)} \<inter> g) \<subseteq> fullG (G\<^sub>1\<^sup>=)" 
+      using m1(2) par1 
+      apply (auto simp: left\<^sub>r_def left_def)
+      apply (subgoal_tac "((g, l), g'a, l') \<in> {m. fst m \<in> v} \<inter> g'")
+      apply blast
+      apply auto
+      done
+    ultimately show ?thesis by blast
   next
-    case (par2 c\<^sub>2')
+    case (par2 g' c\<^sub>2')
     obtain M\<^sub>1 where m1: "P\<^sub>1 \<subseteq> M\<^sub>1" "stable R\<^sub>1 M\<^sub>1" "R\<^sub>1,G\<^sub>1 \<turnstile> M\<^sub>1 {c\<^sub>1} Q\<^sub>1" using par
       by (meson g_stable_preE)
-    obtain P M\<^sub>2 where m2: "P\<^sub>2 \<subseteq> P" "R\<^sub>2,G\<^sub>2 \<turnstile>\<^sub>A P { \<alpha> } M\<^sub>2" "R\<^sub>2,G\<^sub>2 \<turnstile> M\<^sub>2 {c\<^sub>2'} Q\<^sub>2"
-      using par2 par(4)[OF par2(2)] by blast
-    hence "R\<^sub>1 \<inter> R\<^sub>2,G\<^sub>1 \<union> G\<^sub>2 \<turnstile> M\<^sub>1 \<inter> M\<^sub>2 {c'} Q\<^sub>1 \<inter> Q\<^sub>2" using par2 m1 par by blast
-    moreover have "R\<^sub>2 \<inter> R\<^sub>1,G\<^sub>1 \<union> G\<^sub>2 \<turnstile>\<^sub>A P \<inter> M\<^sub>1 { \<alpha> } M\<^sub>2 \<inter> M\<^sub>1" 
-      using atomic_frameI[OF m2(2) m1(2) par(5)] by blast
-    ultimately show ?thesis using m2(1) m1(1) by (metis inf_commute inf_mono)
+    obtain M\<^sub>2 v where m2: "P\<^sub>2 \<subseteq> wp v g' M\<^sub>2" "({m. fst m \<in> v} \<inter> g') \<subseteq> fullG (G\<^sub>2\<^sup>=)" "R\<^sub>2,G\<^sub>2 \<turnstile> M\<^sub>2 {c\<^sub>2'} Q\<^sub>2"
+      using par2 par(4)[OF par2(3)] by blast
+    hence "R\<^sub>1 \<inter> R\<^sub>2,G\<^sub>1 \<union> G\<^sub>2 \<turnstile> left M\<^sub>1 \<inter> right M\<^sub>2 {c'} left Q\<^sub>1 \<inter> right Q\<^sub>2" 
+      using par2 m1 par by blast
+    moreover have "left P\<^sub>1 \<inter> right P\<^sub>2 \<subseteq> wp (right v) g (left M\<^sub>1 \<inter> right M\<^sub>2)" 
+      using par2 m2(1,2) m1(1,2) par.hyps(5)
+      unfolding left_def right_def right\<^sub>r_def wp_def stable_def
+      apply auto
+      apply (subgoal_tac "((gb, rb), aa, r') \<in> fullG (R\<^sub>1\<^sup>=)")
+      apply (subgoal_tac "(gb, lb) \<in> M\<^sub>1")
+      apply auto
+      apply (subgoal_tac "((gb, rb), aa, r') \<in> {((g, l), g', l').
+           (g, g') \<in> G\<^sub>2 \<or> g = g'}")
+      apply auto
+      apply (subgoal_tac "((gb, rb), aa, r') \<in> {m. fst m \<in> v} \<inter> g'")
+      apply blast
+      by auto
+    moreover have "({m. fst m \<in> (right v)} \<inter> g) \<subseteq> fullG (G\<^sub>2\<^sup>=)" 
+      using m2(2) par2 
+      apply (auto simp: right\<^sub>r_def right_def)
+      apply (subgoal_tac "((g, r), g'a, r') \<in> {m. fst m \<in> v} \<inter> g'")
+      apply blast
+      apply auto
+      done
+    ultimately show ?thesis by blast
   qed 
 next
   case (conseq R G P c Q P' R' G' Q')
-  thus ?case using rules.conseq atomic_conseqI by (smt dual_order.trans order_refl)
-next
+  then obtain v M where m: "P \<subseteq> wp v g M" "({m. fst m \<in> v} \<inter> g) \<subseteq> fullG (G\<^sup>=)" "R,G \<turnstile> M {c'} Q" by metis
+  hence "P' \<subseteq> wp v g M" "({m. fst m \<in> v} \<inter> g) \<subseteq> fullG (G'\<^sup>=)" using conseq by auto
+  moreover have "R',G' \<turnstile> M {c'} Q'" using conseq m rules.conseq by auto
+  ultimately show ?case by auto
+(*next
   case (frame R G P c Q R' M')
-  then obtain P' M where "P \<subseteq> P'" "R,G \<turnstile>\<^sub>A P' {\<alpha>} M" "R,G \<turnstile> M {c'} Q" by metis
-  thus ?case using rules.frame atomic_frameI frame(3,4) by blast
+  then obtain P' M where "P \<subseteq> P'" "R,G \<turnstile>\<^sub>A P' {\<alpha>\<llangle>r\<rrangle>} M" "R,G \<turnstile> M {c'} Q" by metis
+  thus ?case using rules.frame atomic_frameI frame(3,4) by blast *)
 next
   case (thread R G P c Q)
-  then show ?case using stepI[OF thread(3,1)] thread(2) indep_stepI[OF thread(2,3)] by auto 
+  hence "local c" using local_only by auto
+  then obtain r \<alpha> where \<alpha>: "c \<mapsto>[r,\<alpha>] c'" "g = leaf\<^sub>r (eval \<alpha>\<llangle>r\<rrangle>)" using thread gexec_localE
+    by blast
+  then obtain P' M where act: "P \<subseteq> P'" "R,G \<turnstile>\<^sub>A P' {\<alpha>\<llangle>r\<rrangle>} M" "R,G \<turnstile> leaf M {c'} leaf Q"
+    using stepI[OF \<alpha>(1) thread(1)] indep_stepI[OF thread(2) \<alpha>(1)] by blast
+  moreover have  "(({m. fst m \<in> leaf (vc \<alpha>\<llangle>r\<rrangle>)}) \<inter> g) \<subseteq> fullG (G\<^sup>=)" using \<alpha>(2) act(2) 
+    apply (auto simp: atomic_rule_def leaf_def leaf\<^sub>r_def eval_def)
+    by blast
+  moreover have "leaf P \<subseteq> wp (leaf (vc \<alpha>\<llangle>r\<rrangle>)) g (leaf M)"
+    using \<alpha>(2) act(1,2) 
+    by (auto simp: atomic_rule_def leaf\<^sub>r_def eval_def wp_def leaf_def)
+  ultimately show ?case by blast
 qed
 
 section \<open>Soundness\<close>
 
 text \<open>All traces that start with a program c\<close>
-fun cp :: "('a,'b) com \<Rightarrow> ('a,'b) config list \<Rightarrow> bool"
+fun cp :: "('a,'b,'c) com \<Rightarrow> ('a,'b,'c) config list \<Rightarrow> bool"
   where "cp c t = (t \<in> transitions \<and> fst (t ! 0) = c)"
 
 text \<open>All traces that satisfy a precondition in their first state\<close>
-fun pre :: "'b pred \<Rightarrow> ('a,'b) config list \<Rightarrow> bool"
+fun pre :: "('b,'c) gpred \<Rightarrow> ('a,'b,'c) config list \<Rightarrow> bool"
   where 
     "pre P (s#t) = (snd s \<in> P)" | 
     "pre P [] = True"
 
 text \<open>All traces that satisfy a postcondition in their final state given termination\<close>
-fun post :: "'b pred \<Rightarrow> ('a,'b) config list \<Rightarrow> bool"
+fun post :: "('b,'c) gpred \<Rightarrow> ('a,'b,'c) config list \<Rightarrow> bool"
   where 
     "post Q [s] = (fst s = Nil \<longrightarrow> snd s \<in> Q)" | 
     "post Q (s#t) = post Q t" | 
     "post Q [] = True"
 
 text \<open>All traces where program steps satisfy a guarantee\<close>
-fun gurn :: "'b rpred \<Rightarrow> ('a,'b) config list \<Rightarrow> bool"
+fun gurn :: "('b,'c) rpred \<Rightarrow> ('a,'b,'c) config list \<Rightarrow> bool"
   where
-    "gurn G (s#s'#t) = (gurn G (s'#t) \<and> (s -c\<rightarrow> s' \<longrightarrow> (snd s, snd s') \<in> G\<^sup>=))" |
+    "gurn G (s#s'#t) = (gurn G (s'#t) \<and> (s -c\<rightarrow> s' \<longrightarrow> (fst (snd s), fst (snd s')) \<in> G\<^sup>=))" |
     "gurn G _ = True"
 
 text \<open>All traces where environment steps satisfy a rely\<close>
-fun rely :: "'b rpred \<Rightarrow> ('a,'b) config list \<Rightarrow> bool"
+fun rely :: "('b,'c) rpred \<Rightarrow> ('a,'b,'c) config list \<Rightarrow> bool"
   where
-    "rely R (s#s'#t) = (rely R (s'#t) \<and> (s -e\<rightarrow> s' \<longrightarrow> (snd s, snd s') \<in> R))" |
+    "rely R (s#s'#t) = (rely R (s'#t) \<and> (s -e\<rightarrow> s' \<longrightarrow> (snd s, snd s') \<in> fullR R))" |
     "rely R _ = True"
 
 text \<open>Validity of the rely/guarantee judgements\<close>
 definition validity ("\<Turnstile> _ SAT [_, _, _, _]" [60,0,0,0,0] 45) 
   where "\<Turnstile> c SAT [P, R, G, Q] \<equiv> \<forall>t. cp c t \<and> pre P t \<and> rely R t \<longrightarrow> post Q t \<and> gurn G t"
+
 
 subsection \<open>Soundness Proof\<close>
 
@@ -298,11 +351,20 @@ next
   thus ?case using env by (auto simp: stable_def)
 next
   case (prg s s' t)
-  then obtain \<alpha> r \<alpha>' where \<alpha>: "c \<mapsto>[\<alpha>,r,\<alpha>'] (fst s')" "(snd s,snd s') \<in> eval \<alpha>" by auto
-  then obtain P' M where p: "P \<subseteq> P'" "R,G \<turnstile>\<^sub>A P' {\<alpha>} M" "R,G \<turnstile> M {fst s'} Q"
-    using g_stepI[OF prg(5) \<alpha>(1)] by metis    
-  hence "rely R (s' # t)" "pre M (s' # t)" "(snd s, snd s') \<in> G\<^sup>="
-    using prg \<alpha>(2) apply (auto simp: eval_def atomic_rule_def wp_def) by fastforce+
+  then obtain g where \<alpha>: "c \<mapsto>[g] (fst s')" "(snd s,snd s') \<in> g" by auto
+  then obtain v M where p: "P \<subseteq> wp v g M" "({m. fst m \<in> v} \<inter> g) \<subseteq> fullG (G\<^sup>=)" "R,G \<turnstile> M {fst s'} Q"
+    using g_stepI[OF prg(5) \<alpha>(1)] by auto
+  hence "rely R (s' # t)" "pre M (s' # t)" "(fst (snd s), fst (snd s')) \<in> G\<^sup>="
+    using prg \<alpha>(2)
+    apply (auto simp: wp_def)
+    apply (cases "snd s'", auto)
+    apply (subgoal_tac "(snd s,snd s') \<in> {m. fst m \<in> v} \<inter> g")
+    apply (metis (mono_tags, lifting) Ball_Collect old.prod.case prod.collapse)
+    apply auto
+    apply (subgoal_tac "(snd s,snd s') \<in> {m. fst m \<in> v} \<inter> g")
+    apply (metis (mono_tags, lifting) Ball_Collect old.prod.case prod.collapse)
+    apply auto
+    done
   thus ?case using prg p(3) by auto
 next
   case (sil s s' t)
