Syntax.thy
@@ -4,41 +4,55 @@ begin
 
 chapter \<open>While Language Syntax\<close>
 
+type_synonym 'a seq = "'a list"
+
 text \<open>
 A While language with non-deterministic choice, iteration and parallel composition.
 Also includes special commands for environment steps, which is useful for describing
 refinement properties. These have no evaluation semantics or rules however.
 \<close>
-datatype ('a,'b) com =
+datatype ('a,'b,'c) com =
   Nil
   | Basic "'a"
-  | Rel "'b rel"
-  | Seq "('a,'b) com" "('a,'b) com" (infixr ";" 80)
-  | Choice "('a,'b) com" "('a,'b) com" (infixr "\<sqinter>" 150)
-  | Loop "('a,'b) com" ("_*" [100] 150)
-  | Parallel "('a,'b) com" "('a,'b) com"  (infixr "||" 150)
+  | Seq "('a,'b,'c) com" "('a,'b,'c) com" (infixr ";" 80)
+  | Ord "('a,'b,'c) com" "('a,'b,'c) com" (infixr "\<cdot>" 80)
+  | BigChoice "'a seq set" ("\<Sqinter> _" 150)
+  | Choice "('a,'b,'c) com" "('a,'b,'c) com" (infixr "\<sqinter>" 150)
+  | Loop "('a,'b,'c) com" ("_*" [100] 150)
+  | Parallel "('a,'b,'c) com" "('a,'b,'c) com"  (infixr "||" 150)
+  | Rel "('b \<times> 'c) rel"
+
+text \<open>Convert a sequence to a command\<close>
+fun seq2com
+  where "seq2com [] = Nil" | "seq2com (\<alpha>#t) = Basic \<alpha> \<cdot> seq2com t"
 
 text \<open>Ensure there is no parallelism within a program\<close>
-fun local :: "('a,'b) com \<Rightarrow> bool"
+fun local :: "('a,'b,'c) com \<Rightarrow> bool"
   where 
     "local (c\<^sub>1 || c\<^sub>2) = False" |
     "local (Rel r) = False" |
     "local (c\<^sub>1 ; c\<^sub>2) = (local c\<^sub>1 \<and> local c\<^sub>2)" |    
+    "local (c\<^sub>1 \<cdot> c\<^sub>2) = (local c\<^sub>1 \<and> local c\<^sub>2)" |    
     "local (c\<^sub>1 \<sqinter> c\<^sub>2) = (local c\<^sub>1 \<and> local c\<^sub>2)" |  
     "local (c*) = (local c)" |    
     "local _ = True"
 
 text \<open>Identify all operations in a program\<close>
-fun basics :: "('a,'b) com \<Rightarrow> 'a set"
+fun basics :: "('a,'b,'c) com \<Rightarrow> 'a set"
   where
     "basics (Basic \<beta>) = {\<beta>}" |
     "basics (Seq c\<^sub>1 c\<^sub>2) = basics c\<^sub>1 \<union> basics c\<^sub>2" |
+    "basics (Ord c\<^sub>1 c\<^sub>2) = basics c\<^sub>1 \<union> basics c\<^sub>2" |
     "basics (Choice c\<^sub>1 c\<^sub>2) = basics c\<^sub>1 \<union> basics c\<^sub>2" |
+    "basics (BigChoice S) = (\<Union>s \<in> S. set s)" |
     "basics (Parallel c\<^sub>1 c\<^sub>2) = basics c\<^sub>1 \<union> basics c\<^sub>2" |
     "basics (Loop c) = basics c" |
     "basics _ = {}"
 
+abbreviation fullR
+  where "fullR R \<equiv> {((g,l),(g',l)) | l g g'. (g,g') \<in> R}"
+
 abbreviation Env
-  where "Env R \<equiv> Rel (R\<^sup>*)"
+  where "Env R \<equiv> Rel (fullR (R\<^sup>*))"
 
 end
