Refine.thy
@@ -13,7 +13,7 @@ locale refine = soundness +
   fixes act_ref :: "'a \<Rightarrow> 'a \<Rightarrow> bool"
   assumes ref_vc: "act_ref \<alpha> \<beta> \<Longrightarrow> vc \<alpha> \<subseteq> vc \<beta>"
   assumes ref_beh: "act_ref \<alpha> \<beta> \<Longrightarrow> beh \<beta> \<subseteq> beh \<alpha>"
-  assumes ref_re: "act_ref \<gamma>\<^sub>1 \<gamma>\<^sub>2 \<Longrightarrow> \<gamma>\<^sub>2 \<hookleftarrow> \<alpha>\<langle>\<gamma>\<^sub>2\<rangle> \<Longrightarrow> act_ref \<beta> \<alpha> \<Longrightarrow> \<gamma>\<^sub>1 \<hookleftarrow> \<beta>\<langle>\<gamma>\<^sub>1\<rangle> \<and> act_ref \<beta>\<langle>\<gamma>\<^sub>1\<rangle> \<alpha>\<langle>\<gamma>\<^sub>2\<rangle>"
+  assumes ref_re: "act_ref \<gamma>\<^sub>1 \<gamma>\<^sub>2 \<Longrightarrow> act_ref \<beta> \<alpha> \<Longrightarrow> act_ref \<beta>\<langle>\<gamma>\<^sub>1\<rangle> \<alpha>\<langle>\<gamma>\<^sub>2\<rangle>"
 
 context refine
 begin
@@ -48,22 +48,22 @@ next
 qed auto
 
 lemma fwd_ref:
-  assumes "lang_ref c\<^sub>1 c\<^sub>2" "\<alpha>' < c\<^sub>2 <\<^sub>c \<alpha>" "act_ref \<beta> \<alpha>"
-  obtains \<beta>' where "\<beta>' < c\<^sub>1 <\<^sub>c \<beta>" "act_ref \<beta>' \<alpha>'"
+  assumes "lang_ref c\<^sub>1 c\<^sub>2" "act_ref \<beta> \<alpha>"
+  shows "act_ref \<beta>\<llangle>c\<^sub>1\<rrangle> \<alpha>\<llangle>c\<^sub>2\<rrangle>"
   using assms
-proof (induct c\<^sub>1 c\<^sub>2 arbitrary: \<alpha> \<beta> \<alpha>' rule: lang_ref.induct)
+proof (induct c\<^sub>1 c\<^sub>2 arbitrary: \<alpha> \<beta> rule: lang_ref.induct)
   case (2 \<gamma>\<^sub>1 \<gamma>\<^sub>2)
   then show ?case using ref_re by force
 next
   case (3 c\<^sub>1 c\<^sub>2 c\<^sub>3 c\<^sub>4)
-  then show ?case by (smt lang_ref.simps(3) reorder_com.simps(3))
+  then show ?case by (smt lang_ref.simps(3) fwd_com.simps(3))
 qed auto
 
 lemma lang_ref_prg:
-  assumes "lang_ref c\<^sub>1 c\<^sub>2" "c\<^sub>2 \<mapsto>[\<alpha>,r,\<alpha>'] c\<^sub>2'" 
-  obtains c\<^sub>1' \<beta> r' \<beta>' where "c\<^sub>1 \<mapsto>[\<beta>,r',\<beta>'] c\<^sub>1'" "lang_ref c\<^sub>1' c\<^sub>2'" "act_ref \<beta> \<alpha>"
+  assumes "lang_ref c\<^sub>1 c\<^sub>2" "c\<^sub>2 \<mapsto>[r,\<alpha>] c\<^sub>2'" 
+  obtains c\<^sub>1' \<beta> r' where "c\<^sub>1 \<mapsto>[r',\<beta>] c\<^sub>1'" "lang_ref c\<^sub>1' c\<^sub>2'" "act_ref \<beta>\<llangle>r'\<rrangle> \<alpha>\<llangle>r\<rrangle>"
   using assms 
-proof (induct c\<^sub>1 c\<^sub>2 arbitrary: c\<^sub>2' \<alpha> r \<alpha>' rule: lang_ref.induct)
+proof (induct c\<^sub>1 c\<^sub>2 arbitrary: c\<^sub>2' \<alpha> r rule: lang_ref.induct)
   case (2 \<alpha>'' \<beta>)
   then show ?case by fastforce
 next
@@ -73,12 +73,12 @@ next
     case (seq c\<^sub>3')
     then show ?thesis using 3(1)[OF _ _ seq(2)] 3(3,4) by fastforce
   next
-    case (ooo \<alpha>'' c c\<^sub>4')
+    case (ooo r' c\<^sub>4')
     show ?thesis
     proof (rule 3(2)[OF _ _ ooo(3)], goal_cases)
-      case (1 \<beta> r' \<beta>' c\<^sub>1')
-      obtain \<beta>' where "\<beta>' < c\<^sub>1 <\<^sub>c \<beta>" "act_ref \<beta>' \<alpha>" 
-        using fwd_ref[OF _ ooo(4) 1(3), of c\<^sub>1] 3(4) by auto
+      case (1 r'' \<beta> c\<^sub>2')
+      hence "act_ref \<beta>\<llangle>c\<^sub>1 ; r''\<rrangle> \<alpha>\<llangle>c\<^sub>3 ; r'\<rrangle>" 
+        using fwd_ref[OF _ 1(3), of c\<^sub>1] 3(4) by auto
       then show ?case using 3(3) 3(4,5) 1 ooo by (meson lang_ref.simps(3) semantics.ooo)
     next
       case 2
@@ -101,11 +101,11 @@ next
   thus ?case using env by (auto simp: stable_def)
 next
   case (prg s s' t)
-  then obtain \<alpha> r \<alpha>' where \<alpha>: "c\<^sub>2 \<mapsto>[\<alpha>,r,\<alpha>'] (fst s')" "(snd s,snd s') \<in> eval \<alpha>" by auto
-  then obtain \<beta> r' \<beta>' c\<^sub>1' where \<beta>: 
-      "c\<^sub>1 \<mapsto>[\<beta>,r',\<beta>'] c\<^sub>1'" "lang_ref c\<^sub>1' (fst s')" "vc \<beta> \<subseteq> vc \<alpha>" "beh \<alpha> \<subseteq> beh \<beta>" 
+  then obtain \<alpha> r where \<alpha>: "c\<^sub>2 \<mapsto>[r,\<alpha>] (fst s')" "(snd s,snd s') \<in> eval \<alpha>\<llangle>r\<rrangle>" by auto
+  then obtain \<beta> r' c\<^sub>1' where \<beta>: 
+      "c\<^sub>1 \<mapsto>[r',\<beta>] c\<^sub>1'" "lang_ref c\<^sub>1' (fst s')" "vc \<beta>\<llangle>r'\<rrangle> \<subseteq> vc \<alpha>\<llangle>r\<rrangle>" "beh \<alpha>\<llangle>r\<rrangle> \<subseteq> beh \<beta>\<llangle>r'\<rrangle>" 
     using lang_ref_prg ref_vc ref_beh prg(8) by metis
-  then obtain P' M where p: "P \<subseteq> P'" "R,G \<turnstile>\<^sub>A P' {\<beta>} M" "R,G \<turnstile> M {c\<^sub>1'} Q"
+  then obtain P' M where p: "P \<subseteq> P'" "R,G \<turnstile>\<^sub>A P' {\<beta>\<llangle>r'\<rrangle>} M" "R,G \<turnstile> M {c\<^sub>1'} Q"
     using g_stepI[OF prg(5) \<beta>(1)] by metis
   hence "rely R (s' # t)" "pre M (s' # t)" "(snd s, snd s') \<in> G\<^sup>="
     using prg(6,7) \<alpha>(2) \<beta>(3,4) unfolding eval_def atomic_rule_def wp_def by auto blast+
